ulib/FStar.Classical.fst
@@ -1,175 +1,190 @@
 module FStar.Classical
 open FStar.Squash
 
-val give_witness: #a:Type -> a -> Lemma (ensures a)
+val give_witness: #a: Type -> a -> Lemma (ensures a)
 let give_witness #a x = return_squash x
 
-val get_squashed (#b a:Type) : Pure a (requires (a /\ a == squash b)) (ensures (fun _ -> True))
+val get_squashed: #b: Type -> a: Type ->
+  Pure a (requires (a /\ a == squash b)) (ensures (fun _ -> True))
 let get_squashed #b a =
   let p = get_proof a in
   join_squash #b p
 
-val get_equality (#t:Type) (a b:t) : Pure (a == b) (requires (a == b)) (ensures (fun _ -> True))
+val get_equality: #t: Type -> a: t -> b: t ->
+  Pure (a == b) (requires (a == b)) (ensures (fun _ -> True))
 let get_equality #t a b = get_squashed #(equals a b) (a == b)
 
-val get_forall (#a:Type) (p:a -> GTot Type0) : Pure (forall (x:a). p x) (requires (forall (x:a). p x)) (ensures (fun _ -> True))
-let get_forall #a p =
-  get_squashed #(x:a -> GTot (p x)) (forall (x:a). p x)
+val get_forall: #a: Type -> p: (a -> GTot Type0) ->
+  Pure (forall (x: a). p x) (requires (forall (x: a). p x)) (ensures (fun _ -> True))
+let get_forall #a p = get_squashed #(x: a -> GTot (p x)) (forall (x: a). p x)
 
-val impl_to_arrow : #a:Type0 -> #b:Type0 -> impl:(a ==> b) -> sx:squash a -> GTot (squash b)
+val impl_to_arrow: #a: Type0 -> #b: Type0 -> impl: (a ==> b) -> sx: squash a -> GTot (squash b)
 let impl_to_arrow #a #b impl sx =
-  bind_squash #(a -> GTot b) impl (fun f ->
-  bind_squash sx (fun x ->
-  return_squash (f x)))
+  bind_squash #(a -> GTot b) impl (fun f -> bind_squash sx (fun x -> return_squash (f x)))
 
-val arrow_to_impl : #a:Type0 -> #b:Type0 -> f:(squash a -> GTot (squash b)) -> GTot (a ==> b)
+val arrow_to_impl: #a: Type0 -> #b: Type0 -> f: (squash a -> GTot (squash b)) -> GTot (a ==> b)
 let arrow_to_impl #a #b f = squash_double_arrow (return_squash (fun x -> f (return_squash x)))
 
 (* TODO: Maybe this should move to FStar.Squash.fst *)
-val forall_intro_gtot  : #a:Type -> #p:(a -> GTot Type) -> $f:(x:a -> GTot (p x)) -> Tot (squash (forall (x:a). p x))
-let forall_intro_gtot #a #p $f = 
-    let id (#a:Type) (x:a) = x in
-    let h : (x:a -> GTot (id (p x))) = fun x -> f x in
-    return_squash #(forall (x:a). id (p x)) ()
+val forall_intro_gtot: #a: Type -> #p: (a -> GTot Type) -> $f: (x: a -> GTot (p x)) ->
+  Tot (squash (forall (x: a). p x))
+let forall_intro_gtot #a #p $f =
+  let id (#a: Type) (x: a) = x in
+  let h: (x: a -> GTot (id (p x))) = fun x -> f x in
+  return_squash #(forall (x: a). id (p x)) ()
 
-val lemma_forall_intro_gtot  : #a:Type -> #p:(a -> GTot Type) -> $f:(x:a -> GTot (p x)) -> Lemma (forall (x:a). p x)
-let lemma_forall_intro_gtot #a #p $f = 
-    let aux () : u:unit{forall x. p x} = forall_intro_gtot #a #p f in
-    aux ()
+val lemma_forall_intro_gtot: #a: Type -> #p: (a -> GTot Type) -> $f: (x: a -> GTot (p x)) ->
+  Lemma (forall (x: a). p x)
+let lemma_forall_intro_gtot #a #p $f =
+  let aux () : u: unit{forall x. p x} = forall_intro_gtot #a #p f in
+  aux ()
 
-val gtot_to_lemma  : #a:Type -> #p:(a -> GTot Type) -> $f:(x:a -> GTot (p x)) -> x:a -> Lemma (p x)
+val gtot_to_lemma: #a: Type -> #p: (a -> GTot Type) -> $f: (x: a -> GTot (p x)) -> x: a ->
+  Lemma (p x)
 let gtot_to_lemma #a #p $f x = give_proof #(p x) (return_squash (f x))
 
-val lemma_to_squash_gtot  : #a:Type -> #p:(a -> GTot Type) -> $f:(x:a -> Lemma (p x)) -> x:a -> GTot (squash (p x))
+val lemma_to_squash_gtot: #a: Type -> #p: (a -> GTot Type) -> $f: (x: a -> Lemma (p x)) -> x: a ->
+  GTot (squash (p x))
 let lemma_to_squash_gtot #a #p $f x = f x; get_proof (p x)
 
-val forall_intro_squash_gtot  : #a:Type -> #p:(a -> GTot Type) -> $f:(x:a -> GTot (squash (p x))) -> Tot (squash (forall (x:a). p x))
+val forall_intro_squash_gtot: 
+  #a: Type ->
+  #p: (a -> GTot Type) ->
+  $f: (x: a -> GTot (squash (p x))) ->
+  Tot (squash (forall (x: a). p x))
 let forall_intro_squash_gtot #a #p $f =
-  bind_squash #(x:a -> GTot (p x)) #(forall (x:a). p x)
-	      (squash_double_arrow #a #p (return_squash f))
-	      (fun f -> lemma_forall_intro_gtot #a #p f)
+  bind_squash #(x: a -> GTot (p x))
+    #(forall (x: a). p x)
+    (squash_double_arrow #a #p (return_squash f))
+    (fun f -> lemma_forall_intro_gtot #a #p f)
 
 //This one seems more generally useful than the one above
-val forall_intro_squash_gtot_join  : #a:Type -> #p:(a -> GTot Type) -> $f:(x:a -> GTot (squash (p x))) -> Tot (forall (x:a). p x)
+val forall_intro_squash_gtot_join: 
+  #a: Type ->
+  #p: (a -> GTot Type) ->
+  $f: (x: a -> GTot (squash (p x))) ->
+  Tot (forall (x: a). p x)
 let forall_intro_squash_gtot_join #a #p $f =
-  join_squash
-    (bind_squash #(x:a -> GTot (p x)) #(forall (x:a). p x)
-	      (squash_double_arrow #a #p (return_squash f))
-	      (fun f -> lemma_forall_intro_gtot #a #p f))
+  join_squash (bind_squash #(x: a -> GTot (p x))
+        #(forall (x: a). p x)
+        (squash_double_arrow #a #p (return_squash f))
+        (fun f -> lemma_forall_intro_gtot #a #p f))
 
-val forall_intro  : #a:Type -> #p:(a -> GTot Type) -> $f:(x:a -> Lemma (p x)) -> Lemma (forall (x:a). p x)
-let forall_intro #a #p $f = 
-    let aux () : (u:unit{forall x. p x}) = forall_intro_squash_gtot (lemma_to_squash_gtot #a #p f) in
-    aux ()
+val forall_intro: #a: Type -> #p: (a -> GTot Type) -> $f: (x: a -> Lemma (p x)) ->
+  Lemma (forall (x: a). p x)
+let forall_intro #a #p $f =
+  let aux () : (u: unit{forall x. p x}) = forall_intro_squash_gtot (lemma_to_squash_gtot #a #p f) in
+  aux ()
 
-val forall_intro'  : #a:Type -> #p:(a -> GTot Type) -> f:(x:a -> Lemma (p x)) -> Lemma (forall (x:a). p x)
+val forall_intro': #a: Type -> #p: (a -> GTot Type) -> f: (x: a -> Lemma (p x)) ->
+  Lemma (forall (x: a). p x)
 let forall_intro' #a #p f = forall_intro f
 
 (* val forall_elim : #a:Type -> #p:(a -> GTot Type) -> (forall (x:a). p x) -> v:a -> Lemma (p v) *)
 
 (* Some basic stuff, should be moved to FStar.Squash, probably *)
-let forall_intro_2 (#a:Type) (#b:(a -> Type)) (#p:(x:a -> b x -> GTot Type0))
-                  ($f: (x:a -> y:b x -> Lemma (p x y)))
-  : Lemma (forall (x:a) (y:b x). p x y)
-  = let g : x:a -> Lemma (forall (y:b x). p x y) = fun x -> forall_intro (f x) in
-    forall_intro g
+let forall_intro_2
+  (#a: Type) (#b: (a -> Type)) (#p: (x: a -> b x -> GTot Type0))
+  ($f: (x: a -> y: b x -> Lemma (p x y)))
+  : Lemma (forall (x: a) (y: b x). p x y) =
+  let g: x: a -> Lemma (forall (y: b x). p x y) = fun x -> forall_intro (f x) in
+  forall_intro g
 
-let forall_intro_3 (#a:Type) (#b:(a -> Type)) (#c:(x:a -> y:b x -> Type)) (#p:(x:a -> y:b x -> z:c x y -> Type0))
-		  ($f: (x:a -> y:b x -> z:c x y -> Lemma (p x y z)))
-  : Lemma (forall (x:a) (y:b x) (z:c x y). p x y z)
-  = let g : x:a -> Lemma (forall (y:b x) (z:c x y). p x y z) = fun x -> forall_intro_2 (f x) in
-    forall_intro g
+let forall_intro_3
+  (#a: Type) (#b: (a -> Type)) (#c: (x: a -> y: b x -> Type))
+  (#p: (x: a -> y: b x -> z: c x y -> Type0)) ($f: (x: a -> y: b x -> z: c x y -> Lemma (p x y z)))
+  : Lemma (forall (x: a) (y: b x) (z: c x y). p x y z) =
+  let g: x: a -> Lemma (forall (y: b x) (z: c x y). p x y z) = fun x -> forall_intro_2 (f x) in
+  forall_intro g
 
-let exists_intro (#a:Type) (p:(a -> Type)) (witness:a)
-  : Lemma (requires (p witness))
-	  (ensures (exists (x:a). p x))
-  = ()
+let exists_intro (#a: Type) (p: (a -> Type)) (witness: a)
+  : Lemma (requires (p witness)) (ensures (exists (x: a). p x)) = ()
 
-let forall_to_exists (#a:Type) (#p:(a -> Type)) (#r:Type) ($f:(x:a -> Lemma (p x ==> r)))
-  : Lemma ((exists (x:a). p x) ==> r)
-  = forall_intro f
+let forall_to_exists (#a: Type) (#p: (a -> Type)) (#r: Type) ($f: (x: a -> Lemma (p x ==> r)))
+  : Lemma ((exists (x: a). p x) ==> r) = forall_intro f
 
-let forall_to_exists_2 (#a:Type) (#p:(a -> Type)) (#b:Type) (#q:(b -> Type)) (#r:Type)
-		 ($f:(x:a -> y:b -> Lemma ((p x /\ q y) ==> r)))
-  : Lemma (((exists (x:a). p x) /\ (exists (y:b). q y)) ==> r)
-  = forall_intro_2 f
+let forall_to_exists_2
+  (#a: Type) (#p: (a -> Type)) (#b: Type) (#q: (b -> Type)) (#r: Type)
+  ($f: (x: a -> y: b -> Lemma ((p x /\ q y) ==> r)))
+  : Lemma (((exists (x: a). p x) /\ (exists (y: b). q y)) ==> r) = forall_intro_2 f
 
-let impl_intro_gtot (#p:Type0) (#q:Type0) ($f:p -> GTot q) : GTot (p ==> q) = return_squash f
+let impl_intro_gtot (#p: Type0) (#q: Type0) ($f: (p -> GTot q)) : GTot (p ==> q) = return_squash f
 
-let impl_intro (#p:Type0) (#q:Type0) ($f: p -> Lemma q) : Lemma (p ==> q)  =
-    give_witness #(p ==> q) (squash_double_arrow (return_squash (lemma_to_squash_gtot f)))
+let impl_intro (#p: Type0) (#q: Type0) ($f: (p -> Lemma q)) : Lemma (p ==> q) =
+  give_witness #(p ==> q) (squash_double_arrow (return_squash (lemma_to_squash_gtot f)))
 
-val exists_elim: goal:Type -> #a:Type -> #p:(a -> Type) -> $have:squash (exists (x:a). p x) -> f:(x:a{p x} -> GTot (squash goal)) ->
+val exists_elim: 
+  goal: Type ->
+  #a: Type ->
+  #p: (a -> Type) ->
+  $have: squash (exists (x: a). p x) ->
+  f: (x: a{p x} -> GTot (squash goal)) ->
   Lemma goal
 let exists_elim goal #a #p have f =
   let open FStar.Squash in
-  bind_squash #_ #goal (join_squash have) (fun (| x, pf |) -> return_squash pf; f x)
+  bind_squash #_ #goal (join_squash have) (fun (| x , pf |) -> return_squash pf; f x)
 
-let move_requires (#a:Type) (#p:a -> Type) (#q:a -> Type)
-  ($f:(x:a -> Lemma (requires (p x)) (ensures (q x)))) (x:a)
+let move_requires
+  (#a: Type) (#p: (a -> Type)) (#q: (a -> Type))
+  ($f: (x: a -> Lemma (requires (p x)) (ensures (q x)))) (x: a)
   : Lemma (p x ==> q x) =
-      give_proof
-        (bind_squash (get_proof (l_or (p x) (~(p x))))
-        (fun (b : l_or (p x) (~(p x))) ->
-          bind_squash b (fun (b' : c_or (p x) (~(p x))) ->
-            match b' with
-            | Left hp -> give_witness hp; f x; get_proof (p x ==> q x)
-            | Right hnp -> give_witness hnp
-          )))
+  give_proof (bind_squash (get_proof (l_or (p x) (~(p x))))
+        (fun (b: l_or (p x) (~(p x))) ->
+            bind_squash b
+              (fun (b': c_or (p x) (~(p x))) ->
+                  match b' with
+                  | Left hp -> give_witness hp; f x; get_proof (p x ==> q x)
+                  | Right hnp -> give_witness hnp)))
 
-val forall_impl_intro :
-  #a:Type ->
-  #p:(a -> GTot Type) ->
-  #q:(a -> GTot Type) ->
-  $f:(x:a -> (squash(p x)) -> Lemma (q x)) ->
+val forall_impl_intro: 
+  #a: Type ->
+  #p: (a -> GTot Type) ->
+  #q: (a -> GTot Type) ->
+  $f: (x: a -> (squash (p x)) -> Lemma (q x)) ->
   Lemma (forall x. p x ==> q x)
 let forall_impl_intro #a #p #q $f =
-  let f' (x:a) : Lemma (requires (p x)) (ensures (q x)) = f x (get_proof (p x)) in
+  let f' (x: a) : Lemma (requires (p x)) (ensures (q x)) = f x (get_proof (p x)) in
   forall_intro (move_requires f')
 
 // Thanks KM, CH and SZ
-val impl_intro_gen
-  (#p: Type0)
-  (#q: (h: squash p) -> Tot Type0)
-  (f: (x: squash p) -> Lemma (q ()))
-: Lemma (p ==> q ())
+val impl_intro_gen: 
+  #p: Type0 ->
+  #q: (h: squash p -> Tot Type0) ->
+  f: (x: squash p -> Lemma (q ())) ->
+  Lemma (p ==> q ())
 let impl_intro_gen #p #q f =
-  let g () : Lemma
-    (requires p)
-    (ensures (p ==> q ()))
-  =
-   give_proof #(q ()) (f (get_proof p))
-  in
+  let g () : Lemma (requires p) (ensures (p ==> q ())) = give_proof #(q ()) (f (get_proof p)) in
   move_requires g ()
 
-val ghost_lemma: #a:Type -> #p:(a -> GTot Type0) -> #q:(a -> unit -> GTot Type0) ->
-  $f:(x:a -> Ghost unit (p x) (q x)) -> Lemma (forall (x:a). p x ==> q x ())
+val ghost_lemma: 
+  #a: Type ->
+  #p: (a -> GTot Type0) ->
+  #q: (a -> unit -> GTot Type0) ->
+  $f: (x: a -> Ghost unit (p x) (q x)) ->
+  Lemma (forall (x: a). p x ==> q x ())
 let ghost_lemma #a #p #q $f =
- let lem : x:a -> Lemma (p x ==> q x ()) =
-  (fun x ->
-      (* basically, the same as above *)
-      give_proof
-        (bind_squash (get_proof (l_or (p x) (~(p x))))
-        (fun (b : l_or (p x) (~(p x))) ->
-          bind_squash b (fun (b' : c_or (p x) (~(p x))) ->
-            match b' with
-            | Left hp -> give_witness hp; f x; get_proof (p x ==> q x ())
-            | Right hnp -> give_witness hnp
-          ))))
- in forall_intro lem
- 
+  let lem: x: a -> Lemma (p x ==> q x ()) =
+    (fun x ->
+        (* basically, the same as above *)
+        give_proof (bind_squash (get_proof (l_or (p x) (~(p x))))
+              (fun (b: l_or (p x) (~(p x))) ->
+                  bind_squash b
+                    (fun (b': c_or (p x) (~(p x))) ->
+                        match b' with
+                        | Left hp -> give_witness hp; f x; get_proof (p x ==> q x ())
+                        | Right hnp -> give_witness hnp))))
+  in
+  forall_intro lem
+
 let or_elim
-  (#l #r: Type0)
-  (#goal: (squash (l \/ r) -> Tot Type0))
-  (hl: squash l -> Lemma (goal ()))
-  (hr: squash r -> Lemma (goal ()))
-: Lemma
-  ((l \/ r) ==> goal ())
-= impl_intro_gen #l #(fun _ -> goal ()) hl;
+  (#l: Type0) (#r: Type0) (#goal: (squash (l \/ r) -> Tot Type0))
+  (hl: (squash l -> Lemma (goal ()))) (hr: (squash r -> Lemma (goal ())))
+  : Lemma ((l \/ r) ==> goal ()) =
+  impl_intro_gen #l #(fun _ -> goal ()) hl;
   impl_intro_gen #r #(fun _ -> goal ()) hr
 
 ////////////////////////////////////////////////////////////////////////////////
 (* the most standard variant of excluded middle is provable by SMT *)
-val excluded_middle : p:Type -> Lemma (requires (True))
-                                     (ensures (p \/ ~p))
-let excluded_middle (p:Type) = ()
+val excluded_middle: p: Type -> Lemma (requires (True)) (ensures (p \/ ~p))
+let excluded_middle (p: Type) = ()
+
