ulib/FStar.Integers.fst
@@ -16,23 +16,22 @@ type width =
   | W128
   | Winfinite
 
-let fixed_width = w:width{w <> Winfinite}
+let fixed_width = w: width{w <> Winfinite}
 
-let nat_of_width = function
-  | W8   -> Some 8
-  | W16  -> Some 16
-  | W31  -> Some 31
-  | W32  -> Some 32
-  | W63  -> Some 63
-  | W64  -> Some 64
+let nat_of_width =
+  function
+  | W8 -> Some 8
+  | W16 -> Some 16
+  | W31 -> Some 31
+  | W32 -> Some 32
+  | W63 -> Some 63
+  | W64 -> Some 64
   | W128 -> Some 128
   | Winfinite -> None
 
-let nat_of_fixed_width (w:fixed_width) =
-  match nat_of_width w with
-  | Some v -> v
+let nat_of_fixed_width (w: fixed_width) = match nat_of_width w with | Some v -> v
 
-let int_t (s:signedness) (w:width) : Tot Type0 =
+let int_t (s: signedness) (w: width) : Tot Type0 =
   match s, w with
   | Unsigned, Winfinite -> nat
   | Unsigned, W8 -> FStar.UInt8.t
@@ -52,284 +51,270 @@ let int_t (s:signedness) (w:width) : Tot Type0 =
   | Signed, W128 -> FStar.Int128.t
 
 abstract
-let nat_size (x:int) : Type =
-  x >= 0
-let reveal_nat_size x
-  : Lemma (nat_size x <==> x >= 0)
-          [SMTPat (nat_size x)]
-  = ()
+let nat_size (x: int) : Type = x >= 0
+let reveal_nat_size x : Lemma (nat_size x <==> x >= 0) [SMTPat (nat_size x)] = ()
 
 abstract
-let uint_size (x:int) (n:nat) : Type =
-    FStar.UInt.size x n
-let reveal_uint_size x n
-  : Lemma (uint_size x n <==> FStar.UInt.size x n)
-          [SMTPat (uint_size x n)]
-  = ()
+let uint_size (x: int) (n: nat) : Type = FStar.UInt.size x n
+let reveal_uint_size x n : Lemma (uint_size x n <==> FStar.UInt.size x n) [SMTPat (uint_size x n)] =
+  ()
 
 abstract
-let int_size (x:int) (n:pos) : Type =
-    FStar.Int.size x n
-let reveal_int_size x n
-  : Lemma (int_size x n <==> FStar.Int.size x n)
-          [SMTPat (int_size x n)]
-  = ()
+let int_size (x: int) (n: pos) : Type = FStar.Int.size x n
+let reveal_int_size x n : Lemma (int_size x n <==> FStar.Int.size x n) [SMTPat (int_size x n)] = ()
 
-let within_bounds (s:signedness) (w:width) (x:int) =
+let within_bounds (s: signedness) (w: width) (x: int) =
   match s, nat_of_width w with
-  | Signed,   None   -> True
-  | Unsigned, None   -> nat_size x
-  | Signed  , Some n -> int_size x n
+  | Signed, None -> True
+  | Unsigned, None -> nat_size x
+  | Signed, Some n -> int_size x n
   | Unsigned, Some n -> uint_size x n
 
-let v (#s:signedness) (#w:width) (x:int_t s w)
-  : Tot (y:int_t Signed Winfinite{normalize (within_bounds s w y)})
-  = match s with
-    | Unsigned ->
-      (match w with
-       | Winfinite -> (x <: nat)
-       | W8 -> FStar.UInt8.v x
-       | W16 -> FStar.UInt16.v x
-       | W31 -> FStar.UInt31.v x
-       | W32 -> FStar.UInt32.v x
-       | W63 -> FStar.UInt63.v x
-       | W64 -> FStar.UInt64.v x
-       | W128 -> FStar.UInt128.v x)
-    | Signed ->
-      (match w with
-       | Winfinite -> x
-       | W8 -> FStar.Int8.v x
-       | W16 -> FStar.Int16.v x
-       | W31 -> FStar.Int31.v x
-       | W32 -> FStar.Int32.v x
-       | W63 -> FStar.Int63.v x
-       | W64 -> FStar.Int64.v x
-       | W128 -> FStar.Int128.v x)
-
-let u   (#s:signedness) (#w:width)
-        (x:int_t Signed Winfinite{normalize (within_bounds s w x)})
-  : Tot (y:int_t s w{normalize (v x == v y)})
-  = match s with
-    | Unsigned ->
-      (match w with
-       | Winfinite -> (x <: nat)
-       | W8 -> FStar.UInt8.uint_to_t x
-       | W16 -> FStar.UInt16.uint_to_t x
-       | W31 -> FStar.UInt31.uint_to_t x
-       | W32 -> FStar.UInt32.uint_to_t x
-       | W63 -> FStar.UInt63.uint_to_t x
-       | W64 -> FStar.UInt64.uint_to_t x
-       | W128 -> FStar.UInt128.uint_to_t x)
-    | Signed ->
-      (match w with
-       | Winfinite -> x
-       | W8 -> FStar.Int8.int_to_t x
-       | W16 -> FStar.Int16.int_to_t x
-       | W31 -> FStar.Int31.int_to_t x
-       | W32 -> FStar.Int32.int_to_t x
-       | W63 -> FStar.Int63.int_to_t x
-       | W64 -> FStar.Int64.int_to_t x
-       | W128 -> FStar.Int128.int_to_t x)
-
-abstract let cast (#s:signedness) (#s':signedness)
-         (#w:width)      (#w':width)
-         (from:int_t s w{normalize (within_bounds s' w' (v from))})
-   : Tot (to:int_t s' w'{normalize (v from == v to)})
-   = u (v from)
-
-unfold
-let ( + ) (#s:signedness) (#w:width)
-          (x:int_t s w)
-          (y:int_t s w{normalize (within_bounds s w (v x + v y))})
-  : Tot   (z:int_t s w{normalize (v z = v x + v y)})
-  = match s, w with
-    | _, Winfinite -> x + y
-    | Unsigned, W8   -> FStar.UInt8.(x +^ y)
-    | Unsigned, W16  -> FStar.UInt16.(x +^ y)
-    | Unsigned, W31  -> FStar.UInt31.(x +^ y)
-    | Unsigned, W32  -> FStar.UInt32.(x +^ y)
-    | Unsigned, W63  -> FStar.UInt63.(x +^ y)
-    | Unsigned, W64  -> FStar.UInt64.(x +^ y)
-    | Unsigned, W128 -> FStar.UInt128.(x +^ y)
-    | Signed, W8   -> FStar.Int8.(x +^ y)
-    | Signed, W16  -> FStar.Int16.(x +^ y)
-    | Signed, W31  -> FStar.Int31.(x +^ y)
-    | Signed, W32  -> FStar.Int32.(x +^ y)
-    | Signed, W63  -> FStar.Int63.(x +^ y)
-    | Signed, W64  -> FStar.Int64.(x +^ y)
-    | Signed, W128 -> FStar.Int128.(x +^ y)
-
-unfold
-let ( +? ) (#w:width)
-           (x:int_t Unsigned w)
-           (y:int_t Unsigned w)
-  : Tot    (z:int_t Unsigned w{normalize (within_bounds Unsigned w (v x + v y) ==> v z = v x + v y)})
-  = match w with
-    | Winfinite -> x + y
-    | W8 -> FStar.UInt8.(x +?^ y)
-    | W16 -> FStar.UInt16.(x +?^ y)
-    | W31 -> FStar.UInt31.(x +?^ y)
-    | W32 -> FStar.UInt32.(x +?^ y)
-    | W63 -> FStar.UInt63.(x +?^ y)
-    | W64 -> FStar.UInt64.(x +?^ y)
-    | W128 -> FStar.UInt128.(x +?^ y)
-
-let modulo (s:signedness) (x:int) (y:pos{s=Signed ==> y%2=0}) =
+let v (#s: signedness) (#w: width) (x: int_t s w)
+  : Tot (y: int_t Signed Winfinite {normalize (within_bounds s w y)}) =
   match s with
-  | Unsigned ->  x % y
-  | _ -> FStar.Int.(x @% y)
+  | Unsigned ->
+    (match w with
+      | Winfinite -> (x <: nat)
+      | W8 -> FStar.UInt8.v x
+      | W16 -> FStar.UInt16.v x
+      | W31 -> FStar.UInt31.v x
+      | W32 -> FStar.UInt32.v x
+      | W63 -> FStar.UInt63.v x
+      | W64 -> FStar.UInt64.v x
+      | W128 -> FStar.UInt128.v x)
+  | Signed ->
+    (match w with
+      | Winfinite -> x
+      | W8 -> FStar.Int8.v x
+      | W16 -> FStar.Int16.v x
+      | W31 -> FStar.Int31.v x
+      | W32 -> FStar.Int32.v x
+      | W63 -> FStar.Int63.v x
+      | W64 -> FStar.Int64.v x
+      | W128 -> FStar.Int128.v x)
+
+let u (#s: signedness) (#w: width) (x: int_t Signed Winfinite {normalize (within_bounds s w x)})
+  : Tot (y: int_t s w {normalize (v x == v y)}) =
+  match s with
+  | Unsigned ->
+    (match w with
+      | Winfinite -> (x <: nat)
+      | W8 -> FStar.UInt8.uint_to_t x
+      | W16 -> FStar.UInt16.uint_to_t x
+      | W31 -> FStar.UInt31.uint_to_t x
+      | W32 -> FStar.UInt32.uint_to_t x
+      | W63 -> FStar.UInt63.uint_to_t x
+      | W64 -> FStar.UInt64.uint_to_t x
+      | W128 -> FStar.UInt128.uint_to_t x)
+  | Signed ->
+    (match w with
+      | Winfinite -> x
+      | W8 -> FStar.Int8.int_to_t x
+      | W16 -> FStar.Int16.int_to_t x
+      | W31 -> FStar.Int31.int_to_t x
+      | W32 -> FStar.Int32.int_to_t x
+      | W63 -> FStar.Int63.int_to_t x
+      | W64 -> FStar.Int64.int_to_t x
+      | W128 -> FStar.Int128.int_to_t x)
+
+abstract
+let cast
+  (#s: signedness) (#s': signedness) (#w: width) (#w': width)
+  (from: int_t s w {normalize (within_bounds s' w' (v from))})
+  : Tot (to: int_t s' w' {normalize (v from == v to)}) = u (v from)
 
 unfold
-let ( +% ) (#w:fixed_width)
-           (x:int_t Unsigned w)
-           (y:int_t Unsigned w)
-  : Tot    (z:int_t Unsigned w{v z == modulo Unsigned (v x + v y) (pow2 (nat_of_fixed_width w))})
-  = match w with
-    | W8 -> FStar.UInt8.(x +%^ y)
-    | W16 -> FStar.UInt16.(x +%^ y)
-    | W31 -> FStar.UInt31.(x +%^ y)
-    | W32 -> FStar.UInt32.(x +%^ y)
-    | W63 -> FStar.UInt63.(x +%^ y)
-    | W64 -> FStar.UInt64.(x +%^ y)
-    | W128 -> FStar.UInt128.(x +%^ y)
+let op_Plus
+  (#s: signedness) (#w: width) (x: int_t s w)
+  (y: int_t s w {normalize (within_bounds s w (v x + v y))})
+  : Tot (z: int_t s w {normalize (v z = v x + v y)}) =
+  match s, w with
+  | _, Winfinite -> x + y
+  | Unsigned, W8 -> let open FStar.UInt8 in x +^ y
+  | Unsigned, W16 -> let open FStar.UInt16 in x +^ y
+  | Unsigned, W31 -> let open FStar.UInt31 in x +^ y
+  | Unsigned, W32 -> let open FStar.UInt32 in x +^ y
+  | Unsigned, W63 -> let open FStar.UInt63 in x +^ y
+  | Unsigned, W64 -> let open FStar.UInt64 in x +^ y
+  | Unsigned, W128 -> let open FStar.UInt128 in x +^ y
+  | Signed, W8 -> let open FStar.Int8 in x +^ y
+  | Signed, W16 -> let open FStar.Int16 in x +^ y
+  | Signed, W31 -> let open FStar.Int31 in x +^ y
+  | Signed, W32 -> let open FStar.Int32 in x +^ y
+  | Signed, W63 -> let open FStar.Int63 in x +^ y
+  | Signed, W64 -> let open FStar.Int64 in x +^ y
+  | Signed, W128 -> let open FStar.Int128 in x +^ y
 
 unfold
-let op_Subtraction (#s:signedness) (#w:width)
-                   (x:int_t s w)
-                   (y:int_t s w{within_bounds s w (v x - v y)})
-    : Tot          (z:int_t s w{v z = v x - v y})
-  = match s, w with
-    | _, Winfinite -> x - y
-    | Unsigned, W8 -> FStar.UInt8.(x -^ y)
-    | Unsigned, W16 -> FStar.UInt16.(x -^ y)
-    | Unsigned, W31 -> FStar.UInt31.(x -^ y)
-    | Unsigned, W32 -> FStar.UInt32.(x -^ y)
-    | Unsigned, W63 -> FStar.UInt63.(x -^ y)
-    | Unsigned, W64 -> FStar.UInt64.(x -^ y)
-    | Unsigned, W128 -> FStar.UInt128.(x -^ y)
-    | Signed, W8 -> FStar.Int8.(x -^ y)
-    | Signed, W16 -> FStar.Int16.(x -^ y)
-    | Signed, W31 -> FStar.Int31.(x -^ y)
-    | Signed, W32 -> FStar.Int32.(x -^ y)
-    | Signed, W63 -> FStar.Int63.(x -^ y)
-    | Signed, W64 -> FStar.Int64.(x -^ y)
-    | Signed, W128 -> FStar.Int128.(x -^ y)
+let op_Plus_Question (#w: width) (x: int_t Unsigned w) (y: int_t Unsigned w)
+  : Tot (z: int_t Unsigned w {normalize (within_bounds Unsigned w (v x + v y) ==> v z = v x + v y)}) =
+  match w with
+  | Winfinite -> x + y
+  | W8 -> let open FStar.UInt8 in x +?^ y
+  | W16 -> let open FStar.UInt16 in x +?^ y
+  | W31 -> let open FStar.UInt31 in x +?^ y
+  | W32 -> let open FStar.UInt32 in x +?^ y
+  | W63 -> let open FStar.UInt63 in x +?^ y
+  | W64 -> let open FStar.UInt64 in x +?^ y
+  | W128 -> let open FStar.UInt128 in x +?^ y
+
+let modulo (s: signedness) (x: int) (y: pos{s = Signed ==> y % 2 = 0}) =
+  match s with
+  | Unsigned -> x % y
+  | _ -> let open FStar.Int in x @% y
 
 unfold
-let op_Subtraction_Question
-        (#w:width)
-        (x:int_t Unsigned w)
-        (y:int_t Unsigned w)
-  : Tot (z:int_t Unsigned w{within_bounds Unsigned w (v x - v y) ==> v z = v x - v y})
-  = match w with
-    | Winfinite -> if v x - v y >= 0 then x - y else 0
-    | W8 -> FStar.UInt8.(x -?^ y)
-    | W16 -> FStar.UInt16.(x -?^ y)
-    | W31 -> FStar.UInt31.(x -?^ y)
-    | W32 -> FStar.UInt32.(x -?^ y)
-    | W63 -> FStar.UInt63.(x -?^ y)
-    | W64 -> FStar.UInt64.(x -?^ y)
-    | W128 -> FStar.UInt128.(x -?^ y)
+let op_Plus_Percent (#w: fixed_width) (x: int_t Unsigned w) (y: int_t Unsigned w)
+  : Tot (z: int_t Unsigned w {v z == modulo Unsigned (v x + v y) (pow2 (nat_of_fixed_width w))}) =
+  match w with
+  | W8 -> let open FStar.UInt8 in x +%^ y
+  | W16 -> let open FStar.UInt16 in x +%^ y
+  | W31 -> let open FStar.UInt31 in x +%^ y
+  | W32 -> let open FStar.UInt32 in x +%^ y
+  | W63 -> let open FStar.UInt63 in x +%^ y
+  | W64 -> let open FStar.UInt64 in x +%^ y
+  | W128 -> let open FStar.UInt128 in x +%^ y
 
 unfold
-let op_Subtraction_Percent
-         (#w:fixed_width)
-         (x:int_t Unsigned w)
-         (y:int_t Unsigned w)
-  : Tot  (z:int_t Unsigned w{v z = modulo Unsigned (v x - v y) (pow2 (nat_of_fixed_width w))})
-  = match w with
-    | W8 -> FStar.UInt8.(x -%^ y)
-    | W16 -> FStar.UInt16.(x -%^ y)
-    | W31 -> FStar.UInt31.(x -%^ y)
-    | W32 -> FStar.UInt32.(x -%^ y)
-    | W63 -> FStar.UInt63.(x -%^ y)
-    | W64 -> FStar.UInt64.(x -%^ y)
-    | W128 -> FStar.UInt128.(x -%^ y)
+let op_Subtraction
+  (#s: signedness) (#w: width) (x: int_t s w) (y: int_t s w {within_bounds s w (v x - v y)})
+  : Tot (z: int_t s w {v z = v x - v y}) =
+  match s, w with
+  | _, Winfinite -> x - y
+  | Unsigned, W8 -> let open FStar.UInt8 in x -^ y
+  | Unsigned, W16 -> let open FStar.UInt16 in x -^ y
+  | Unsigned, W31 -> let open FStar.UInt31 in x -^ y
+  | Unsigned, W32 -> let open FStar.UInt32 in x -^ y
+  | Unsigned, W63 -> let open FStar.UInt63 in x -^ y
+  | Unsigned, W64 -> let open FStar.UInt64 in x -^ y
+  | Unsigned, W128 -> let open FStar.UInt128 in x -^ y
+  | Signed, W8 -> let open FStar.Int8 in x -^ y
+  | Signed, W16 -> let open FStar.Int16 in x -^ y
+  | Signed, W31 -> let open FStar.Int31 in x -^ y
+  | Signed, W32 -> let open FStar.Int32 in x -^ y
+  | Signed, W63 -> let open FStar.Int63 in x -^ y
+  | Signed, W64 -> let open FStar.Int64 in x -^ y
+  | Signed, W128 -> let open FStar.Int128 in x -^ y
+
+unfold
+let op_Subtraction_Question (#w: width) (x: int_t Unsigned w) (y: int_t Unsigned w)
+  : Tot (z: int_t Unsigned w {within_bounds Unsigned w (v x - v y) ==> v z = v x - v y}) =
+  match w with
+  | Winfinite -> if v x - v y >= 0 then x - y else 0
+  | W8 -> let open FStar.UInt8 in x -?^ y
+  | W16 -> let open FStar.UInt16 in x -?^ y
+  | W31 -> let open FStar.UInt31 in x -?^ y
+  | W32 -> let open FStar.UInt32 in x -?^ y
+  | W63 -> let open FStar.UInt63 in x -?^ y
+  | W64 -> let open FStar.UInt64 in x -?^ y
+  | W128 -> let open FStar.UInt128 in x -?^ y
+
+unfold
+let op_Subtraction_Percent (#w: fixed_width) (x: int_t Unsigned w) (y: int_t Unsigned w)
+  : Tot (z: int_t Unsigned w {v z = modulo Unsigned (v x - v y) (pow2 (nat_of_fixed_width w))}) =
+  match w with
+  | W8 -> let open FStar.UInt8 in x -%^ y
+  | W16 -> let open FStar.UInt16 in x -%^ y
+  | W31 -> let open FStar.UInt31 in x -%^ y
+  | W32 -> let open FStar.UInt32 in x -%^ y
+  | W63 -> let open FStar.UInt63 in x -%^ y
+  | W64 -> let open FStar.UInt64 in x -%^ y
+  | W128 -> let open FStar.UInt128 in x -%^ y
 
 open FStar.Mul
 
 unfold
-let ( * ) (#s:signedness) (#w:width{w <> W128})
-          (x:int_t s w)
-          (y:int_t s w{within_bounds s w (v x * v y)})
-  : Tot   (z:int_t s w{v z = v x * v y})
-  = match s, w with
-    | _, Winfinite -> x * y
-    | Unsigned, W8 -> FStar.UInt8.(x *^ y)
-    | Unsigned, W16 -> FStar.UInt16.(x *^ y)
-    | Unsigned, W31 -> FStar.UInt31.(x *^ y)
-    | Unsigned, W32 -> FStar.UInt32.(x *^ y)
-    | Unsigned, W63 -> FStar.UInt63.(x *^ y)
-    | Unsigned, W64 -> FStar.UInt64.(x *^ y)
-    | Signed, W8 -> FStar.Int8.(x *^ y)
-    | Signed, W16 -> FStar.Int16.(x *^ y)
-    | Signed, W31 -> FStar.Int31.(x *^ y)
-    | Signed, W32 -> FStar.Int32.(x *^ y)
-    | Signed, W63 -> FStar.Int63.(x *^ y)
-    | Signed, W64 -> FStar.Int64.(x *^ y)
-    | Signed, W128 -> FStar.Int128.(x *^ y)
+let op_Star
+  (#s: signedness) (#w: width{w <> W128}) (x: int_t s w)
+  (y: int_t s w {within_bounds s w (v x * v y)})
+  : Tot (z: int_t s w {v z = v x * v y}) =
+  match s, w with
+  | _, Winfinite -> x * y
+  | Unsigned, W8 -> let open FStar.UInt8 in x *^ y
+  | Unsigned, W16 -> let open FStar.UInt16 in x *^ y
+  | Unsigned, W31 -> let open FStar.UInt31 in x *^ y
+  | Unsigned, W32 -> let open FStar.UInt32 in x *^ y
+  | Unsigned, W63 -> let open FStar.UInt63 in x *^ y
+  | Unsigned, W64 -> let open FStar.UInt64 in x *^ y
+  | Signed, W8 -> let open FStar.Int8 in x *^ y
+  | Signed, W16 -> let open FStar.Int16 in x *^ y
+  | Signed, W31 -> let open FStar.Int31 in x *^ y
+  | Signed, W32 -> let open FStar.Int32 in x *^ y
+  | Signed, W63 -> let open FStar.Int63 in x *^ y
+  | Signed, W64 -> let open FStar.Int64 in x *^ y
+  | Signed, W128 -> let open FStar.Int128 in x *^ y
 
 unfold
-let ( *? ) (#w:width{w <> W128})
-           (x:int_t Unsigned w)
-           (y:int_t Unsigned w)
-  : Tot    (z:int_t Unsigned w{within_bounds Unsigned w (v x * v y) ==> v z = v x * v y})
-  = match w with
-    | Winfinite -> x * y
-    | W8 -> FStar.UInt8.(x *?^ y)
-    | W16 -> FStar.UInt16.(x *?^ y)
-    | W31 -> FStar.UInt31.(x *?^ y)
-    | W32 -> FStar.UInt32.(x *?^ y)
-    | W63 -> FStar.UInt63.(x *?^ y)
-    | W64 -> FStar.UInt64.(x *?^ y)
+let op_Star_Question (#w: width{w <> W128}) (x: int_t Unsigned w) (y: int_t Unsigned w)
+  : Tot (z: int_t Unsigned w {within_bounds Unsigned w (v x * v y) ==> v z = v x * v y}) =
+  match w with
+  | Winfinite -> x * y
+  | W8 -> let open FStar.UInt8 in x *?^ y
+  | W16 -> let open FStar.UInt16 in x *?^ y
+  | W31 -> let open FStar.UInt31 in x *?^ y
+  | W32 -> let open FStar.UInt32 in x *?^ y
+  | W63 -> let open FStar.UInt63 in x *?^ y
+  | W64 -> let open FStar.UInt64 in x *?^ y
 
 unfold
-let ( *% ) (#w:fixed_width{w <> W128})
-           (x:int_t Unsigned w)
-           (y:int_t Unsigned w)
-  : Tot    (z:int_t Unsigned w{v z = modulo Unsigned (v x * v y) (pow2 (nat_of_fixed_width w))})
-  = match w with
-    | W8 -> FStar.UInt8.(x *%^ y)
-    | W16 -> FStar.UInt16.(x *%^ y)
-    | W31 -> FStar.UInt31.(x *%^ y)
-    | W32 -> FStar.UInt32.(x *%^ y)
-    | W63 -> FStar.UInt63.(x *%^ y)
-    | W64 -> FStar.UInt64.(x *%^ y)
-
-unfold let nat        = int_t Unsigned Winfinite
-unfold let uint_8   = int_t Unsigned W8
-unfold let uint_16  = int_t Unsigned W16
-unfold let uint_31  = int_t Unsigned W31
-unfold let uint_32  = int_t Unsigned W32
-unfold let uint_63  = int_t Unsigned W63
-unfold let uint_64  = int_t Unsigned W64
-
-unfold let int       = int_t Signed Winfinite
-unfold let int_8   = int_t Signed W8
-unfold let int_16  = int_t Signed W16
-unfold let int_31  = int_t Signed W31
-unfold let int_32  = int_t Signed W32
-unfold let int_63  = int_t Signed W63
-unfold let int_64  = int_t Signed W64
-unfold let int_128 = int_t Signed W128
+let op_Star_Percent (#w: fixed_width{w <> W128}) (x: int_t Unsigned w) (y: int_t Unsigned w)
+  : Tot (z: int_t Unsigned w {v z = modulo Unsigned (v x * v y) (pow2 (nat_of_fixed_width w))}) =
+  match w with
+  | W8 -> let open FStar.UInt8 in x *%^ y
+  | W16 -> let open FStar.UInt16 in x *%^ y
+  | W31 -> let open FStar.UInt31 in x *%^ y
+  | W32 -> let open FStar.UInt32 in x *%^ y
+  | W63 -> let open FStar.UInt63 in x *%^ y
+  | W64 -> let open FStar.UInt64 in x *%^ y
 
 unfold
-let ok (#s:signedness) (#w:width)
-       (op:(int_t Signed Winfinite
-          -> int_t Signed Winfinite
-          -> int_t Signed Winfinite))
-       (x:int_t s w)
-       (y:int_t s w)
-   = normalize (within_bounds s w (op (v x) (v y)))
+let nat = int_t Unsigned Winfinite
+unfold
+let uint_8 = int_t Unsigned W8
+unfold
+let uint_16 = int_t Unsigned W16
+unfold
+let uint_31 = int_t Unsigned W31
+unfold
+let uint_32 = int_t Unsigned W32
+unfold
+let uint_63 = int_t Unsigned W63
+unfold
+let uint_64 = int_t Unsigned W64
+
+unfold
+let int = int_t Signed Winfinite
+unfold
+let int_8 = int_t Signed W8
+unfold
+let int_16 = int_t Signed W16
+unfold
+let int_31 = int_t Signed W31
+unfold
+let int_32 = int_t Signed W32
+unfold
+let int_63 = int_t Signed W63
+unfold
+let int_64 = int_t Signed W64
+unfold
+let int_128 = int_t Signed W128
+
+unfold
+let ok
+  (#s: signedness) (#w: width)
+  (op: (int_t Signed Winfinite -> int_t Signed Winfinite -> int_t Signed Winfinite)) (x: int_t s w)
+  (y: int_t s w) = normalize (within_bounds s w (op (v x) (v y)))
 ////////////////////////////////////////////////////////////////////////////////
 //Test
 ////////////////////////////////////////////////////////////////////////////////
-let f_int (x:int) (y:int) = x + y
-let f_nat (x:nat) (y:nat) = x + y
-let f_uint_8 (x:uint_8) (y:uint_8{ok (+) x y}) = x + y
-let f_int_16 (x:int_16) (y:int_16{ok (+) x y}) = x + y
-let g (x:uint_32) (y:uint_32{ok ( * ) y y /\ ok (+) x (y * y)}) = x + y * y
-let h (x:Prims.nat) (y:Prims.nat): nat  = u x + u y
+let f_int (x: int) (y: int) = x + y
+let f_nat (x: nat) (y: nat) = x + y
+let f_uint_8 (x: uint_8) (y: uint_8{ok ( + ) x y}) = x + y
+let f_int_16 (x: int_16) (y: int_16{ok ( + ) x y}) = x + y
+let g (x: uint_32) (y: uint_32{ok ( * ) y y /\ ok ( + ) x (y * y)}) = x + y * y
+let h (x: Prims.nat) (y: Prims.nat) : nat = u x + u y
+
 (* TODO: A bit boring ... *)
 (* let op_Slash_Hat = div *)
 (* let op_Percent_Hat = rem *)
