ulib/FStar.Modifies.fst
@@ -7,213 +7,137 @@ module U32 = FStar.UInt32
 
 noeq
 type loc_aux : Type =
-  | LocBuffer:
-    (#t: Type) ->
-    (b: B.buffer t) ->
-    loc_aux
-  | LocUnion:
-    (l1: loc_aux) ->
-    (l2: loc_aux) ->
-    loc_aux
+  | LocBuffer : #t: Type -> b: B.buffer t -> loc_aux
+  | LocUnion : l1: loc_aux -> l2: loc_aux -> loc_aux
 
-let rec loc_aux_in_addr
-  (l: loc_aux)
-  (r: HS.rid)
-  (n: nat)
-: GTot Type0
-  (decreases l)
-= match l with
+let rec loc_aux_in_addr (l: loc_aux) (r: HS.rid) (n: nat) : GTot Type0 (decreases l) =
+  match l with
   | LocUnion l1 l2 -> loc_aux_in_addr l1 r n /\ loc_aux_in_addr l2 r n
-  | LocBuffer b ->
-    B.frameOf b == r /\
-    B.as_addr b == n
+  | LocBuffer b -> B.frameOf b == r /\ B.as_addr b == n
 
 noeq
 type loc' : Type =
-  | Loc:
-      (regions: Ghost.erased (Set.set HS.rid)) ->
-      (addrs: (
-	(r: HS.rid) ->
-	Ghost (Set.set nat)
-	(requires (Set.mem r (Ghost.reveal regions)))
-	(ensures (fun _ -> True))
-      )) ->
-      (aux_addrs: (
-	(r: HS.rid) ->
-	Ghost (Set.set nat)
-	(requires (Set.mem r (Ghost.reveal regions)))
-	(ensures (fun y -> Set.subset (Set.intersect y (addrs r)) Set.empty))
-      )) ->
-      (aux: (
-	(r: HS.rid) ->
-	(n: nat) ->
-	Ghost loc_aux
-	(requires (
-	  Set.mem r (Ghost.reveal regions) /\
-	  Set.mem n (aux_addrs r)
-	))
-	(ensures (fun y ->
-          loc_aux_in_addr y r n
-      )))) ->
-      loc'
+  | Loc : 
+    regions: Ghost.erased (Set.set HS.rid) ->
+    addrs:
+    (r: HS.rid ->
+        Ghost (Set.set nat) (requires (Set.mem r (Ghost.reveal regions))) (ensures (fun _ -> True))) ->
+    aux_addrs:
+    (r: HS.rid ->
+        Ghost (Set.set nat)
+          (requires (Set.mem r (Ghost.reveal regions)))
+          (ensures (fun y -> Set.subset (Set.intersect y (addrs r)) Set.empty))) ->
+    aux:
+    (r: HS.rid -> n: nat ->
+        Ghost loc_aux
+          (requires (Set.mem r (Ghost.reveal regions) /\ Set.mem n (aux_addrs r)))
+          (ensures (fun y -> loc_aux_in_addr y r n))) ->
+    loc'
 
 let loc = loc'
 
-let loc_none = Loc
-  (Ghost.hide (Set.empty))
-  (fun _ -> Set.empty)
-  (fun _ -> Set.empty)
-  (fun _ _ -> false_elim ())
+let loc_none =
+  Loc (Ghost.hide (Set.empty)) (fun _ -> Set.empty) (fun _ -> Set.empty) (fun _ _ -> false_elim ())
 
-let regions_of_loc
-  (s: loc)
-: GTot (Set.set HS.rid)
-= Ghost.reveal (Loc?.regions s)
+let regions_of_loc (s: loc) : GTot (Set.set HS.rid) = Ghost.reveal (Loc?.regions s)
 
-let addrs_of_loc_weak
-  (l: loc)
-  (r: HS.rid)
-: GTot (Set.set nat)
-= if Set.mem r (regions_of_loc l)
-  then Loc?.addrs l r
-  else Set.empty
+let addrs_of_loc_weak (l: loc) (r: HS.rid) : GTot (Set.set nat) =
+  if Set.mem r (regions_of_loc l) then Loc?.addrs l r else Set.empty
 
-let addrs_of_loc_aux
-  (l: loc)
-  (r: HS.rid)
-: GTot (Set.set nat)
-= if Set.mem r (regions_of_loc l)
-  then Loc?.aux_addrs l r
-  else Set.empty
+let addrs_of_loc_aux (l: loc) (r: HS.rid) : GTot (Set.set nat) =
+  if Set.mem r (regions_of_loc l) then Loc?.aux_addrs l r else Set.empty
 
-let addrs_of_loc
-  (l: loc)
-  (r: HS.rid)
-: GTot (Set.set nat)
-= Set.union
-    (addrs_of_loc_weak l r)
-    (addrs_of_loc_aux l r)
+let addrs_of_loc (l: loc) (r: HS.rid) : GTot (Set.set nat) =
+  Set.union (addrs_of_loc_weak l r) (addrs_of_loc_aux l r)
 
-let addrs_of_loc_aux_prop
-  (l: loc)
-  (r: HS.rid)
-: Lemma
-  (Set.subset (Set.intersect (addrs_of_loc_aux l r) (addrs_of_loc_weak l r)) Set.empty)
-  [SMTPatOr [
-    [SMTPat (addrs_of_loc_aux l r)];
-    [SMTPat (addrs_of_loc_weak l r)];
-    [SMTPat (addrs_of_loc l r)];
-  ]]
-= ()
+let addrs_of_loc_aux_prop (l: loc) (r: HS.rid)
+  : Lemma (Set.subset (Set.intersect (addrs_of_loc_aux l r) (addrs_of_loc_weak l r)) Set.empty)
+    [
+      SMTPatOr
+      [
+        [SMTPat (addrs_of_loc_aux l r)];
+        [SMTPat (addrs_of_loc_weak l r)];
+        [SMTPat (addrs_of_loc l r)]
+      ]
+    ] = ()
 
 let loc_union s1 s2 =
   if StrongExcludedMiddle.strong_excluded_middle (s1 == s2)
   then s1
   else
-  let regions1 = Ghost.reveal (Loc?.regions s1) in
-  let regions2 = Ghost.reveal (Loc?.regions s2) in
-  let regions = Set.union regions1 regions2 in
-  let addrs
-    (r: HS.rid)
-  : Ghost (Set.set nat)
-    (requires (Set.mem r regions))
-    (ensures (fun _ -> True))
-  = Set.union
-      (if Set.mem r regions1 then Loc?.addrs s1 r else Set.empty)
-      (if Set.mem r regions2 then Loc?.addrs s2 r else Set.empty)
-  in
-  let aux_addrs
-    (r: HS.rid)
-  : Ghost (Set.set nat)
-    (requires (Set.mem r regions))
-    (ensures (fun y -> Set.subset (Set.intersect y (addrs r)) Set.empty))
-  = Set.intersect
-      (Set.union (addrs_of_loc_aux s1 r) (addrs_of_loc_aux s2 r))
-      (Set.complement (addrs r))
-  in
-  let aux
-    (r: HS.rid)
-    (n: nat)
-  : Ghost loc_aux
-    (requires (Set.mem r regions /\ Set.mem n (aux_addrs r)))
-    (ensures (fun y -> loc_aux_in_addr y r n))
-  = let l1 =
-      if Set.mem r regions1 && Set.mem n (Loc?.aux_addrs s1 r)
-      then Some (Loc?.aux s1 r n)
-      else None
+    let regions1 = Ghost.reveal (Loc?.regions s1) in
+    let regions2 = Ghost.reveal (Loc?.regions s2) in
+    let regions = Set.union regions1 regions2 in
+    let addrs (r: HS.rid)
+      : Ghost (Set.set nat) (requires (Set.mem r regions)) (ensures (fun _ -> True)) =
+      Set.union (if Set.mem r regions1 then Loc?.addrs s1 r else Set.empty)
+        (if Set.mem r regions2 then Loc?.addrs s2 r else Set.empty)
     in
-    let l2 =
-      if Set.mem r regions2 && Set.mem n (Loc?.aux_addrs s2 r)
-      then Some (Loc?.aux s2 r n)
-      else None
+    let aux_addrs (r: HS.rid)
+      : Ghost (Set.set nat)
+        (requires (Set.mem r regions))
+        (ensures (fun y -> Set.subset (Set.intersect y (addrs r)) Set.empty)) =
+      Set.intersect (Set.union (addrs_of_loc_aux s1 r) (addrs_of_loc_aux s2 r))
+        (Set.complement (addrs r))
     in
-    match l1, l2 with
-    | Some l1, Some l2 -> LocUnion l1 l2
-    | Some l1, _ -> l1
-    | _, Some l2 -> l2
-  in
-  Loc
-    (Ghost.hide regions)
-    addrs
-    aux_addrs
-    aux
+    let aux (r: HS.rid) (n: nat)
+      : Ghost loc_aux
+        (requires (Set.mem r regions /\ Set.mem n (aux_addrs r)))
+        (ensures (fun y -> loc_aux_in_addr y r n)) =
+      let l1 =
+        if Set.mem r regions1 && Set.mem n (Loc?.aux_addrs s1 r)
+        then Some (Loc?.aux s1 r n)
+        else None
+      in
+      let l2 =
+        if Set.mem r regions2 && Set.mem n (Loc?.aux_addrs s2 r)
+        then Some (Loc?.aux s2 r n)
+        else None
+      in
+      match l1, l2 with
+      | Some l1, Some l2 -> LocUnion l1 l2
+      | Some l1, _ -> l1
+      | _, Some l2 -> l2
+    in
+    Loc (Ghost.hide regions) addrs aux_addrs aux
 
 let loc_union_idem s = ()
 
 let loc_buffer #t b =
-    Loc
-      (Ghost.hide (Set.singleton (B.frameOf b)))
-      (fun _ -> Set.empty)
-      (fun _ -> Set.singleton (B.as_addr b))
-      (fun _ _ -> LocBuffer b)
+  Loc (Ghost.hide (Set.singleton (B.frameOf b)))
+    (fun _ -> Set.empty)
+    (fun _ -> Set.singleton (B.as_addr b))
+    (fun _ _ -> LocBuffer b)
 
 let loc_addresses r n =
-  Loc
-    (Ghost.hide (Set.singleton r))
-    (fun _ -> n)
-    (fun _ -> Set.empty)
-    (fun _ _ -> false_elim ())
+  Loc (Ghost.hide (Set.singleton r)) (fun _ -> n) (fun _ -> Set.empty) (fun _ _ -> false_elim ())
 
 let loc_regions r =
-  Loc
-    (Ghost.hide r)
+  Loc (Ghost.hide r)
     (fun r' -> if Set.mem r' r then Set.complement Set.empty else Set.empty)
     (fun _ -> Set.empty)
     (fun _ _ -> false_elim ())
 
-let rec loc_aux_includes_buffer
-  (#a: Type)
-  (s: loc_aux)
-  (b: B.buffer a)
-: GTot Type0
-  (decreases s)
-= match s with
+let rec loc_aux_includes_buffer (#a: Type) (s: loc_aux) (b: B.buffer a) : GTot Type0 (decreases s) =
+  match s with
   | LocUnion s1 s2 -> loc_aux_includes_buffer s1 b \/ loc_aux_includes_buffer s2 b
-  | LocBuffer #a0 b0 -> a == a0 /\ b0 `B.includes` b
+  | LocBuffer #a0 b0 -> a == a0 /\ B.includes b0 b
 
-let rec loc_aux_includes
-  (s1 s2: loc_aux)
-: GTot Type0
-  (decreases s2)
-= match s2 with
+let rec loc_aux_includes (s1: loc_aux) (s2: loc_aux) : GTot Type0 (decreases s2) =
+  match s2 with
   | LocUnion s2l s2r -> loc_aux_includes s1 s2l /\ loc_aux_includes s1 s2r
   | LocBuffer b -> loc_aux_includes_buffer s1 b
 
-let rec loc_aux_includes_union_l
-  (s1 s2 s: loc_aux)
-: Lemma
-  (requires (loc_aux_includes s1 s \/ loc_aux_includes s2 s))
-  (ensures (loc_aux_includes (LocUnion s1 s2) s))
-  (decreases s)
-= match s with 
+let rec loc_aux_includes_union_l (s1: loc_aux) (s2: loc_aux) (s: loc_aux)
+  : Lemma (requires (loc_aux_includes s1 s \/ loc_aux_includes s2 s))
+    (ensures (loc_aux_includes (LocUnion s1 s2) s))
+    (decreases s) =
+  match s with
   | LocUnion sl sr -> loc_aux_includes_union_l s1 s2 sl; loc_aux_includes_union_l s1 s2 sr
   | _ -> ()
 
-let rec loc_aux_includes_refl
-  (s: loc_aux)
-: Lemma
-  (loc_aux_includes s s)
-= match s with
+let rec loc_aux_includes_refl (s: loc_aux) : Lemma (loc_aux_includes s s) =
+  match s with
   | LocUnion sl sr ->
     loc_aux_includes_refl sl;
     loc_aux_includes_refl sr;
@@ -221,32 +145,23 @@ let rec loc_aux_includes_refl
     loc_aux_includes_union_l sl sr sr
   | _ -> ()
 
-let loc_aux_includes_union_l_r
-  (s s': loc_aux)
-: Lemma
-  (loc_aux_includes (LocUnion s s') s)
-= loc_aux_includes_refl s;
+let loc_aux_includes_union_l_r (s: loc_aux) (s': loc_aux)
+  : Lemma (loc_aux_includes (LocUnion s s') s) =
+  loc_aux_includes_refl s;
   loc_aux_includes_union_l s s' s
 
-let loc_aux_includes_union_l_l
-  (s s': loc_aux)
-: Lemma
-  (loc_aux_includes (LocUnion s' s) s)
-= loc_aux_includes_refl s;
+let loc_aux_includes_union_l_l (s: loc_aux) (s': loc_aux)
+  : Lemma (loc_aux_includes (LocUnion s' s) s) =
+  loc_aux_includes_refl s;
   loc_aux_includes_union_l s' s s
 
-let rec loc_aux_includes_buffer_includes
-  (#a: Type)
-  (s: loc_aux)
-  (b1 b2: B.buffer a)
-: Lemma
-  (requires (loc_aux_includes_buffer s b1 /\ b1 `B.includes` b2))
-  (ensures (loc_aux_includes_buffer s b2))
-  (decreases s)
-= match s with
+let rec loc_aux_includes_buffer_includes (#a: Type) (s: loc_aux) (b1: B.buffer a) (b2: B.buffer a)
+  : Lemma (requires (loc_aux_includes_buffer s b1 /\ B.includes b1 b2))
+    (ensures (loc_aux_includes_buffer s b2))
+    (decreases s) =
+  match s with
   | LocUnion sl sr ->
-    Classical.or_elim
-      #(loc_aux_includes_buffer sl b1)
+    Classical.or_elim #(loc_aux_includes_buffer sl b1)
       #(loc_aux_includes_buffer sr b1)
       #(fun _ -> loc_aux_includes_buffer s b2)
       (fun _ -> loc_aux_includes_buffer_includes sl b1 b2)
@@ -254,102 +169,71 @@ let rec loc_aux_includes_buffer_includes
   | _ -> ()
 
 let rec loc_aux_includes_loc_aux_includes_buffer
-  (#a: Type)
-  (s1 s2: loc_aux)
-  (b: B.buffer a)
-: Lemma
-  (requires (loc_aux_includes s1 s2 /\ loc_aux_includes_buffer s2 b))
-  (ensures (loc_aux_includes_buffer s1 b))
-  (decreases s2)
-= match s2 with
+  (#a: Type) (s1: loc_aux) (s2: loc_aux) (b: B.buffer a)
+  : Lemma (requires (loc_aux_includes s1 s2 /\ loc_aux_includes_buffer s2 b))
+    (ensures (loc_aux_includes_buffer s1 b))
+    (decreases s2) =
+  match s2 with
   | LocUnion s2l s2r ->
-    Classical.or_elim
-      #(loc_aux_includes_buffer s2l b)
+    Classical.or_elim #(loc_aux_includes_buffer s2l b)
       #(loc_aux_includes_buffer s2r b)
       #(fun _ -> loc_aux_includes_buffer s1 b)
       (fun _ -> loc_aux_includes_loc_aux_includes_buffer s1 s2l b)
       (fun _ -> loc_aux_includes_loc_aux_includes_buffer s1 s2r b)
   | LocBuffer b2 -> loc_aux_includes_buffer_includes s1 b2 b
 
-let rec loc_aux_includes_trans
-  (s1 s2 s3: loc_aux)
-: Lemma
-  (requires (loc_aux_includes s1 s2 /\ loc_aux_includes s2 s3))
-  (ensures (loc_aux_includes s1 s3))
-  (decreases s3)
-= match s3 with
-  | LocUnion s3l s3r ->
-    loc_aux_includes_trans s1 s2 s3l;
-    loc_aux_includes_trans s1 s2 s3r
+let rec loc_aux_includes_trans (s1: loc_aux) (s2: loc_aux) (s3: loc_aux)
+  : Lemma (requires (loc_aux_includes s1 s2 /\ loc_aux_includes s2 s3))
+    (ensures (loc_aux_includes s1 s3))
+    (decreases s3) =
+  match s3 with
+  | LocUnion s3l s3r -> loc_aux_includes_trans s1 s2 s3l; loc_aux_includes_trans s1 s2 s3r
   | LocBuffer b -> loc_aux_includes_loc_aux_includes_buffer s1 s2 b
 
 (* the following is necessary because `decreases` messes up 2nd-order unification with `Classical.forall_intro_3` *)
 
-let loc_aux_includes_trans'
-  (s1 s2: loc_aux)
-  (s3: loc_aux)
-: Lemma
-  ((loc_aux_includes s1 s2 /\ loc_aux_includes s2 s3) ==> loc_aux_includes s1 s3)
-= Classical.move_requires (loc_aux_includes_trans s1 s2) s3
+let loc_aux_includes_trans' (s1: loc_aux) (s2: loc_aux) (s3: loc_aux)
+  : Lemma ((loc_aux_includes s1 s2 /\ loc_aux_includes s2 s3) ==> loc_aux_includes s1 s3) =
+  Classical.move_requires (loc_aux_includes_trans s1 s2) s3
 
-let addrs_of_loc_weak_loc_union
-  (l1 l2: loc)
-  (r: HS.rid)
-: Lemma
-  (addrs_of_loc_weak (loc_union l1 l2) r == Set.union (addrs_of_loc_weak l1 r) (addrs_of_loc_weak l2 r))
-  [SMTPat (addrs_of_loc_weak (loc_union l1 l2) r)]
-= assert (Set.equal (addrs_of_loc_weak (loc_union l1 l2) r) (Set.union (addrs_of_loc_weak l1 r) (addrs_of_loc_weak l2 r)))
+let addrs_of_loc_weak_loc_union (l1: loc) (l2: loc) (r: HS.rid)
+  : Lemma
+    (addrs_of_loc_weak (loc_union l1 l2) r ==
+      Set.union (addrs_of_loc_weak l1 r) (addrs_of_loc_weak l2 r))
+    [SMTPat (addrs_of_loc_weak (loc_union l1 l2) r)] =
+  assert (Set.equal (addrs_of_loc_weak (loc_union l1 l2) r)
+        (Set.union (addrs_of_loc_weak l1 r) (addrs_of_loc_weak l2 r)))
 
-let addrs_of_loc_union
-  (l1 l2: loc)
-  (r: HS.rid)
-: Lemma
-  (addrs_of_loc (loc_union l1 l2) r == Set.union (addrs_of_loc l1 r) (addrs_of_loc l2 r))
-  [SMTPat (addrs_of_loc (loc_union l1 l2) r)]
-= assert (Set.equal (addrs_of_loc (loc_union l1 l2) r) (Set.union (addrs_of_loc l1 r) (addrs_of_loc l2 r)))
+let addrs_of_loc_union (l1: loc) (l2: loc) (r: HS.rid)
+  : Lemma (addrs_of_loc (loc_union l1 l2) r == Set.union (addrs_of_loc l1 r) (addrs_of_loc l2 r))
+    [SMTPat (addrs_of_loc (loc_union l1 l2) r)] =
+  assert (Set.equal (addrs_of_loc (loc_union l1 l2) r)
+        (Set.union (addrs_of_loc l1 r) (addrs_of_loc l2 r)))
 
 let loc_includes s1 s2 =
   let regions1 = Ghost.reveal (Loc?.regions s1) in
-  let regions2 = Ghost.reveal (Loc?.regions s2) in (
-    Set.subset regions2 regions1 /\ (
-      forall (r: HS.rid) .
-      Set.subset (addrs_of_loc_weak s2 r) (addrs_of_loc_weak s1 r)
-    ) /\ (
-      forall (r: HS.rid) .
-      Set.subset (addrs_of_loc s2 r) (addrs_of_loc s1 r)
-    ) /\ (
-      forall (r: HS.rid) (n: nat) .
-      (Set.mem r regions2 /\ Set.mem n (addrs_of_loc_aux s2 r) /\ Set.mem n (addrs_of_loc_aux s1 r)) ==>
-      loc_aux_includes (Loc?.aux s1 r n) (Loc?.aux s2 r n)
-  ))
+  let regions2 = Ghost.reveal (Loc?.regions s2) in
+  (Set.subset regions2 regions1 /\
+    (forall (r: HS.rid). Set.subset (addrs_of_loc_weak s2 r) (addrs_of_loc_weak s1 r)) /\
+    (forall (r: HS.rid). Set.subset (addrs_of_loc s2 r) (addrs_of_loc s1 r)) /\
+    (forall (r: HS.rid) (n: nat).
+        (Set.mem r regions2 /\ Set.mem n (addrs_of_loc_aux s2 r) /\
+          Set.mem n (addrs_of_loc_aux s1 r)) ==>
+        loc_aux_includes (Loc?.aux s1 r n) (Loc?.aux s2 r n)))
 
 let loc_includes_refl s =
-  let pre
-    (r: HS.rid)
-    (n: nat)
-  : GTot Type0
-  = Set.mem r (regions_of_loc s) /\
-    Set.mem n (Loc?.aux_addrs s r)
+  let pre (r: HS.rid) (n: nat) : GTot Type0 =
+    Set.mem r (regions_of_loc s) /\ Set.mem n (Loc?.aux_addrs s r)
   in
-  let post
-    (r: HS.rid)
-    (n: nat)
-  : GTot Type0
-  = pre r n /\
-    loc_aux_includes (Loc?.aux s r n) (Loc?.aux s r n)
+  let post (r: HS.rid) (n: nat) : GTot Type0 =
+    pre r n /\ loc_aux_includes (Loc?.aux s r n) (Loc?.aux s r n)
   in
-  let f
-    (r: HS.rid)
-    (n: nat)
-  : Lemma
-    (requires (pre r n))
-    (ensures (post r n))
-  = loc_aux_includes_refl (Loc?.aux s r n)
+  let f (r: HS.rid) (n: nat) : Lemma (requires (pre r n)) (ensures (post r n)) =
+    loc_aux_includes_refl (Loc?.aux s r n)
   in
   Classical.forall_intro_2 (fun r -> Classical.move_requires (f r))
 
-let loc_includes_trans s1 s2 s3 =
-  Classical.forall_intro_3 loc_aux_includes_trans'
+let loc_includes_trans s1 s2 s3 = Classical.forall_intro_3 loc_aux_includes_trans'
 
 let loc_includes_union_r s s1 s2 = ()
 
@@ -357,17 +241,15 @@ let loc_includes_union_l s1 s2 s =
   let u12 = loc_union s1 s2 in
   if StrongExcludedMiddle.strong_excluded_middle (s1 == s2)
   then ()
-  else begin
-    Classical.forall_intro loc_aux_includes_refl;
-    Classical.forall_intro_2 loc_aux_includes_union_l_l;
-    Classical.forall_intro_2 loc_aux_includes_union_l_r;
-    Classical.or_elim
-      #(loc_includes s1 s)
-      #(loc_includes s2 s)
-      #(fun _ -> loc_includes (loc_union s1 s2) s)
-      (fun _ -> loc_includes_trans u12 s1 s)
-      (fun _ -> loc_includes_trans u12 s2 s)
-  end
+  else
+    (Classical.forall_intro loc_aux_includes_refl;
+      Classical.forall_intro_2 loc_aux_includes_union_l_l;
+      Classical.forall_intro_2 loc_aux_includes_union_l_r;
+      Classical.or_elim #(loc_includes s1 s)
+        #(loc_includes s2 s)
+        #(fun _ -> loc_includes (loc_union s1 s2) s)
+        (fun _ -> loc_includes_trans u12 s1 s)
+        (fun _ -> loc_includes_trans u12 s2 s))
 
 let loc_includes_none s = ()
 
@@ -392,190 +274,142 @@ let loc_includes_region_union_l l s1 s2 = ()
 
 #reset-options
 
-
 (* Disjointness of two memory locations *)
 
-let rec loc_aux_disjoint_buffer
-  (l: loc_aux)
-  (#t: Type)
-  (p: B.buffer t)
-: GTot Type0
-  (decreases l)
-= match l with
-  | LocUnion ll lr ->
-    loc_aux_disjoint_buffer ll p /\ loc_aux_disjoint_buffer lr p
+let rec loc_aux_disjoint_buffer (l: loc_aux) (#t: Type) (p: B.buffer t) : GTot Type0 (decreases l) =
+  match l with
+  | LocUnion ll lr -> loc_aux_disjoint_buffer ll p /\ loc_aux_disjoint_buffer lr p
   | LocBuffer b -> B.disjoint b p
 
-let rec loc_aux_disjoint
-  (l1 l2: loc_aux)
-: GTot Type0
-  (decreases l2)
-= match l2 with
-  | LocUnion ll lr ->
-    loc_aux_disjoint l1 ll /\ loc_aux_disjoint l1 lr
-  | LocBuffer b ->
-    loc_aux_disjoint_buffer l1 b
+let rec loc_aux_disjoint (l1: loc_aux) (l2: loc_aux) : GTot Type0 (decreases l2) =
+  match l2 with
+  | LocUnion ll lr -> loc_aux_disjoint l1 ll /\ loc_aux_disjoint l1 lr
+  | LocBuffer b -> loc_aux_disjoint_buffer l1 b
 
-let rec loc_aux_disjoint_union_l
-  (ll1 lr1 l2: loc_aux)
-: Lemma
-  (ensures (loc_aux_disjoint (LocUnion ll1 lr1) l2 <==> (loc_aux_disjoint ll1 l2 /\ loc_aux_disjoint lr1 l2)))
-  (decreases l2)
-= match l2 with
-  | LocUnion ll2 lr2 ->
-    loc_aux_disjoint_union_l ll1 lr1 ll2;
-    loc_aux_disjoint_union_l ll1 lr1 lr2
+let rec loc_aux_disjoint_union_l (ll1: loc_aux) (lr1: loc_aux) (l2: loc_aux)
+  : Lemma
+    (ensures
+      (loc_aux_disjoint (LocUnion ll1 lr1) l2 <==>
+        (loc_aux_disjoint ll1 l2 /\ loc_aux_disjoint lr1 l2))) (decreases l2) =
+  match l2 with
+  | LocUnion ll2 lr2 -> loc_aux_disjoint_union_l ll1 lr1 ll2; loc_aux_disjoint_union_l ll1 lr1 lr2
   | _ -> ()
 
-let loc_aux_disjoint_union_r
-  (l1 ll2 lr2: loc_aux)
-: Lemma
-  (loc_aux_disjoint l1 (LocUnion ll2 lr2) <==> (loc_aux_disjoint l1 ll2 /\ loc_aux_disjoint l1 lr2))
-= ()
+let loc_aux_disjoint_union_r (l1: loc_aux) (ll2: loc_aux) (lr2: loc_aux)
+  : Lemma
+  (loc_aux_disjoint l1 (LocUnion ll2 lr2) <==> (loc_aux_disjoint l1 ll2 /\ loc_aux_disjoint l1 lr2)) =
+  ()
 
-let rec loc_aux_size
-  (l: loc_aux)
-: GTot nat
-= match l with
+let rec loc_aux_size (l: loc_aux) : GTot nat =
+  match l with
   | LocUnion l1 l2 ->
     let n1 = loc_aux_size l1 in
     let n2 = loc_aux_size l2 in
     1 + (if n1 > n2 then n1 else n2)
   | _ -> 0
 
-let rec loc_aux_disjoint_sym
-  (l1 l2: loc_aux)
-: Lemma
-  (ensures (loc_aux_disjoint l1 l2 <==> loc_aux_disjoint l2 l1))
-  (decreases (loc_aux_size l1 + loc_aux_size l2))
-= match l2 with
+let rec loc_aux_disjoint_sym (l1: loc_aux) (l2: loc_aux)
+  : Lemma (ensures (loc_aux_disjoint l1 l2 <==> loc_aux_disjoint l2 l1))
+    (decreases (loc_aux_size l1 + loc_aux_size l2)) =
+  match l2 with
   | LocUnion ll lr ->
     loc_aux_disjoint_union_r l1 ll lr;
     loc_aux_disjoint_sym l1 ll;
     loc_aux_disjoint_sym l1 lr;
     loc_aux_disjoint_union_l ll lr l1
   | _ ->
-    begin match l1 with
+    match l1 with
     | LocUnion ll lr ->
       loc_aux_disjoint_union_l ll lr l2;
       loc_aux_disjoint_sym ll l2;
       loc_aux_disjoint_sym lr l2;
       loc_aux_disjoint_union_r l2 ll lr
     | _ -> ()
-    end
 
 (* Same problem with decreases here *)
 
-let loc_aux_disjoint_sym'
-  (l1 l2: loc_aux)
-: Lemma
-  (loc_aux_disjoint l1 l2 <==> loc_aux_disjoint l2 l1)
-= loc_aux_disjoint_sym l1 l2
+let loc_aux_disjoint_sym' (l1: loc_aux) (l2: loc_aux)
+  : Lemma (loc_aux_disjoint l1 l2 <==> loc_aux_disjoint l2 l1) = loc_aux_disjoint_sym l1 l2
 
-let regions_of_loc_loc_union
-  (s1 s2: loc)
-: Lemma
-  (regions_of_loc (loc_union s1 s2) == regions_of_loc s1 `Set.union` regions_of_loc s2)
-  [SMTPat (regions_of_loc (loc_union s1 s2))]
-= assert (regions_of_loc (loc_union s1 s2) `Set.equal` (regions_of_loc s1 `Set.union` regions_of_loc s2))
+let regions_of_loc_loc_union (s1: loc) (s2: loc)
+  : Lemma (regions_of_loc (loc_union s1 s2) == Set.union (regions_of_loc s1) (regions_of_loc s2))
+    [SMTPat (regions_of_loc (loc_union s1 s2))] =
+  assert (Set.equal (regions_of_loc (loc_union s1 s2))
+        (Set.union (regions_of_loc s1) (regions_of_loc s2)))
 
-let regions_of_loc_monotonic
-  (s1 s2: loc)
-: Lemma
-  (requires (loc_includes s1 s2))
-  (ensures (Set.subset (regions_of_loc s2) (regions_of_loc s1)))
-= ()
+let regions_of_loc_monotonic (s1: loc) (s2: loc)
+  : Lemma (requires (loc_includes s1 s2))
+    (ensures (Set.subset (regions_of_loc s2) (regions_of_loc s1))) = ()
 
-let loc_disjoint'
-  (l1 l2: loc)
-: GTot Type0
-= (forall (r: HS.rid) .
+let loc_disjoint' (l1: loc) (l2: loc) : GTot Type0 =
+  (forall (r: HS.rid).
       Set.subset (Set.intersect (addrs_of_loc_weak l1 r) (addrs_of_loc l2 r)) Set.empty /\
-      Set.subset (Set.intersect (addrs_of_loc l1 r) (addrs_of_loc_weak l2 r)) Set.empty
-  ) /\
-  (forall (r: HS.rid) (n: nat) .
-    (Set.mem r (regions_of_loc l1) /\ Set.mem n (addrs_of_loc_aux l1 r) /\
-     Set.mem r (regions_of_loc l2) /\ Set.mem n (addrs_of_loc_aux l2 r)) ==>
-    loc_aux_disjoint (Loc?.aux l1 r n) (Loc?.aux l2 r n)
-  )
+      Set.subset (Set.intersect (addrs_of_loc l1 r) (addrs_of_loc_weak l2 r)) Set.empty) /\
+  (forall (r: HS.rid) (n: nat).
+      (Set.mem r (regions_of_loc l1) /\ Set.mem n (addrs_of_loc_aux l1 r) /\
+        Set.mem r (regions_of_loc l2) /\ Set.mem n (addrs_of_loc_aux l2 r)) ==>
+      loc_aux_disjoint (Loc?.aux l1 r n) (Loc?.aux l2 r n))
 
 let loc_disjoint = loc_disjoint'
 
-let loc_disjoint_sym l1 l2 =
-  Classical.forall_intro_2 loc_aux_disjoint_sym'
+let loc_disjoint_sym l1 l2 = Classical.forall_intro_2 loc_aux_disjoint_sym'
 
 let loc_disjoint_none_r s = ()
 
 let loc_disjoint_union_r s s1 s2 = ()
 
-let rec loc_aux_disjoint_buffer_includes
-  (l: loc_aux)
-  (#t: Type)
-  (p1: B.buffer t)
-  (p2: B.buffer t)
-: Lemma
-  (requires (loc_aux_disjoint_buffer l p1 /\ p1 `B.includes` p2))
-  (ensures (loc_aux_disjoint_buffer l p2))
-  (decreases l)
-= match l with
+let rec loc_aux_disjoint_buffer_includes (l: loc_aux) (#t: Type) (p1: B.buffer t) (p2: B.buffer t)
+  : Lemma (requires (loc_aux_disjoint_buffer l p1 /\ B.includes p1 p2))
+    (ensures (loc_aux_disjoint_buffer l p2))
+    (decreases l) =
+  match l with
   | LocUnion ll lr ->
     loc_aux_disjoint_buffer_includes ll p1 p2;
     loc_aux_disjoint_buffer_includes lr p1 p2
   | _ -> ()
 
 let rec loc_aux_disjoint_loc_aux_includes_buffer
-  (l1 l2: loc_aux)
-  (#t3: Type)
-  (b3: B.buffer t3)
-: Lemma
-  (requires (loc_aux_disjoint l1 l2 /\ loc_aux_includes_buffer l2 b3))
-  (ensures (loc_aux_disjoint_buffer l1 b3))
-  (decreases l2)
-= match l2 with
+  (l1: loc_aux) (l2: loc_aux) (#t3: Type) (b3: B.buffer t3)
+  : Lemma (requires (loc_aux_disjoint l1 l2 /\ loc_aux_includes_buffer l2 b3))
+    (ensures (loc_aux_disjoint_buffer l1 b3))
+    (decreases l2) =
+  match l2 with
   | LocUnion l2l l2r ->
-    Classical.or_elim
-      #(loc_aux_includes_buffer l2l b3)
+    Classical.or_elim #(loc_aux_includes_buffer l2l b3)
       #(loc_aux_includes_buffer l2r b3)
       #(fun _ -> loc_aux_disjoint_buffer l1 b3)
       (fun _ -> loc_aux_disjoint_loc_aux_includes_buffer l1 l2l b3)
       (fun _ -> loc_aux_disjoint_loc_aux_includes_buffer l1 l2r b3)
   | LocBuffer b2 -> loc_aux_disjoint_buffer_includes l1 b2 b3
 
-let rec loc_aux_disjoint_loc_aux_includes
-  (l1 l2 l3: loc_aux)
-: Lemma
-  (requires (loc_aux_disjoint l1 l2 /\ loc_aux_includes l2 l3))
-  (ensures (loc_aux_disjoint l1 l3))
-  (decreases l3)
-= match l3 with
+let rec loc_aux_disjoint_loc_aux_includes (l1: loc_aux) (l2: loc_aux) (l3: loc_aux)
+  : Lemma (requires (loc_aux_disjoint l1 l2 /\ loc_aux_includes l2 l3))
+    (ensures (loc_aux_disjoint l1 l3))
+    (decreases l3) =
+  match l3 with
   | LocUnion ll3 lr3 ->
     loc_aux_disjoint_loc_aux_includes l1 l2 ll3;
     loc_aux_disjoint_loc_aux_includes l1 l2 lr3
-  | LocBuffer b3 ->
-    loc_aux_disjoint_loc_aux_includes_buffer l1 l2 b3
+  | LocBuffer b3 -> loc_aux_disjoint_loc_aux_includes_buffer l1 l2 b3
 
 let loc_disjoint_includes p1 p2 p1' p2' =
   regions_of_loc_monotonic p1 p1';
   regions_of_loc_monotonic p2 p2';
-  let pre = //A rather brutal way to force inlining of pre and post in VC of the continuation
+  //A rather brutal way to force inlining of pre and post in VC of the continuation
+  let pre =
     (fun r n ->
-      Set.mem r (regions_of_loc p1') /\ Set.mem n (addrs_of_loc_aux p1' r) /\
-      Set.mem r (regions_of_loc p2') /\ Set.mem n (addrs_of_loc_aux p2' r))
-    <: Tot ((r:HS.rid) -> (n:nat) -> GTot Type0)
+        Set.mem r (regions_of_loc p1') /\ Set.mem n (addrs_of_loc_aux p1' r) /\
+        Set.mem r (regions_of_loc p2') /\ Set.mem n (addrs_of_loc_aux p2' r))
+    <:
+    Tot (r: HS.rid -> n: nat -> GTot Type0)
   in
   let post =
-    (fun r n ->
-       pre r n /\
-       loc_aux_disjoint (Loc?.aux p1' r n) (Loc?.aux p2' r n))
-    <: Tot ((r:HS.rid) -> (n:nat) -> GTot Type0)
+    (fun r n -> pre r n /\ loc_aux_disjoint (Loc?.aux p1' r n) (Loc?.aux p2' r n))
+    <:
+    Tot (r: HS.rid -> n: nat -> GTot Type0)
   in
-  let f
-    (r: HS.rid)
-    (n: nat)
-  : Lemma
-    (requires (pre r n))
-    (ensures (post r n))
-  = let l1 = Loc?.aux p1 r n in
+  let f (r: HS.rid) (n: nat) : Lemma (requires (pre r n)) (ensures (post r n)) =
+    let l1 = Loc?.aux p1 r n in
     let l2 = Loc?.aux p2 r n in
     let l1' = Loc?.aux p1' r n in
     let l2' = Loc?.aux p2' r n in
@@ -599,41 +433,26 @@ let loc_disjoint_regions rs1 rs2 = ()
 
 (** The modifies clause proper *)
 
-let modifies_preserves_mreferences
-  (s: loc)
-  (h1 h2: HS.mem)
-: GTot Type0
-= (forall (t: Type) (pre: Preorder.preorder t) (p: HS.mreference t pre) .
-    let r = HS.frameOf p in (
-      HS.contains h1 p /\
-      (Set.mem r (regions_of_loc s) ==> ~ (Set.mem (HS.as_addr p) (addrs_of_loc s r)))
-    ) ==> (
-      HS.contains h2 p /\
-      HS.sel h2 p == HS.sel h1 p
-  ))
 
-let modifies_preserves_buffers
-  (s: loc)
-  (h1 h2: HS.mem)
-: GTot Type0
-= (forall (t: Type) (b: B.buffer t) .
-    let r = B.frameOf b in
-    let a = B.as_addr b in (
-      B.live h1 b /\
-      B.length b <> 0 /\
-      (Set.mem r (regions_of_loc s) ==> ~ (Set.mem a (addrs_of_loc_weak s r))) /\
-      ((Set.mem r (regions_of_loc s) /\ Set.mem a (addrs_of_loc_aux s r)) ==> loc_aux_disjoint_buffer (Loc?.aux s r a) b)
-    ) ==> (
-      B.live h2 b /\
-      B.as_seq h2 b == B.as_seq h1 b
-  ))
+let modifies_preserves_mreferences (s: loc) (h1: HS.mem) (h2: HS.mem) : GTot Type0 =
+  (forall (t: Type) (pre: Preorder.preorder t) (p: HS.mreference t pre).
+      let r = HS.frameOf p in
+      (HS.contains h1 p /\
+        (Set.mem r (regions_of_loc s) ==> ~(Set.mem (HS.as_addr p) (addrs_of_loc s r)))) ==>
+      (HS.contains h2 p /\ HS.sel h2 p == HS.sel h1 p))
 
-let modifies'
-  (s: loc)
-  (h1 h2: HS.mem)
-: GTot Type0
-= modifies_preserves_mreferences s h1 h2 /\
-  modifies_preserves_buffers s h1 h2
+let modifies_preserves_buffers (s: loc) (h1: HS.mem) (h2: HS.mem) : GTot Type0 =
+  (forall (t: Type) (b: B.buffer t).
+      let r = B.frameOf b in
+      let a = B.as_addr b in
+      (B.live h1 b /\ B.length b <> 0 /\
+        (Set.mem r (regions_of_loc s) ==> ~(Set.mem a (addrs_of_loc_weak s r))) /\
+        ((Set.mem r (regions_of_loc s) /\ Set.mem a (addrs_of_loc_aux s r)) ==>
+          loc_aux_disjoint_buffer (Loc?.aux s r a) b)) ==>
+      (B.live h2 b /\ B.as_seq h2 b == B.as_seq h1 b))
+
+let modifies' (s: loc) (h1: HS.mem) (h2: HS.mem) : GTot Type0 =
+  modifies_preserves_mreferences s h1 h2 /\ modifies_preserves_buffers s h1 h2
 
 let modifies = modifies'
 
@@ -643,25 +462,19 @@ let modifies_buffer_elim #t1 b p h h' = ()
 
 let modifies_refl s h = ()
 
-let loc_aux_disjoint_buffer_loc_aux_includes
-  (l1: loc_aux)
-: Lemma
-  (forall (l2: loc_aux)
-    (t3: Type)
-    (b3: B.buffer t3) .
-  (loc_aux_disjoint_buffer l1 b3 /\ loc_aux_includes l1 l2) ==> loc_aux_disjoint_buffer l2 b3)
-= let f
-  (l2: loc_aux)
-  (t3: Type)
-  (b3: B.buffer t3)
+let loc_aux_disjoint_buffer_loc_aux_includes (l1: loc_aux)
   : Lemma
-    (requires (loc_aux_disjoint_buffer l1 b3 /\ loc_aux_includes l1 l2))
-    (ensures (loc_aux_disjoint_buffer l2 b3))
-  = loc_aux_disjoint_sym (LocBuffer b3) l1;
+  (forall (l2: loc_aux) (t3: Type) (b3: B.buffer t3).
+      (loc_aux_disjoint_buffer l1 b3 /\ loc_aux_includes l1 l2) ==> loc_aux_disjoint_buffer l2 b3) =
+  let f (l2: loc_aux) (t3: Type) (b3: B.buffer t3)
+    : Lemma (requires (loc_aux_disjoint_buffer l1 b3 /\ loc_aux_includes l1 l2))
+      (ensures (loc_aux_disjoint_buffer l2 b3)) =
+    loc_aux_disjoint_sym (LocBuffer b3) l1;
     loc_aux_disjoint_loc_aux_includes (LocBuffer b3) l1 l2;
     loc_aux_disjoint_sym (LocBuffer b3) l2
   in
-  Classical.forall_intro_3 (fun (l2: loc_aux) (t3: Type) (b3: B.buffer t3) -> Classical.move_requires (f l2 t3) b3)
+  Classical.forall_intro_3 (fun (l2: loc_aux) (t3: Type) (b3: B.buffer t3) ->
+        Classical.move_requires (f l2 t3) b3)
 
 #set-options "--z3rlimit 32"
 
@@ -672,14 +485,8 @@ let modifies_loc_includes s1 h h' s2 =
 
 #reset-options
 
-let modifies_trans'
-  (s: loc)
-  (h1 h2: HS.mem)
-  (h3: HS.mem)
-: Lemma
-  (requires (modifies s h1 h2 /\ modifies s h2 h3))
-  (ensures (modifies s h1 h3))
-= ()
+let modifies_trans' (s: loc) (h1: HS.mem) (h2: HS.mem) (h3: HS.mem)
+  : Lemma (requires (modifies s h1 h2 /\ modifies s h2 h3)) (ensures (modifies s h1 h3)) = ()
 
 let modifies_trans s12 h1 h2 s23 h3 =
   let u = loc_union s12 s23 in
@@ -691,84 +498,60 @@ let modifies_trans s12 h1 h2 s23 h3 =
 
 #set-options "--z3rlimit 32"
 
-let modifies_only_live_regions_weak
-  (rs: Set.set HS.rid)
-  (l: loc)
-  (h h' : HS.mem)
-: Lemma
-  (requires (
-    modifies (loc_union (loc_regions rs) l) h h' /\
-    loc_disjoint (loc_regions rs) l /\
-    (forall r . Set.mem r rs ==> (~ (HS.live_region h r)))
-  ))
-  (ensures (modifies l h h'))
-= ()
+let modifies_only_live_regions_weak (rs: Set.set HS.rid) (l: loc) (h: HS.mem) (h': HS.mem)
+  : Lemma
+    (requires
+      (modifies (loc_union (loc_regions rs) l) h h' /\ loc_disjoint (loc_regions rs) l /\
+        (forall r. Set.mem r rs ==> (~(HS.live_region h r))))) (ensures (modifies l h h')) = ()
 
 #reset-options
 
 (* Restrict a set of locations along a set of regions *)
 
-let restrict_to_regions
-  (l: loc)
-  (rs: Set.set HS.rid)
-: GTot loc
-= let (Loc regions addrs aux_addrs aux) = l in
-  Loc
-    (Ghost.hide (Set.intersect (Ghost.reveal regions) rs))
+let restrict_to_regions (l: loc) (rs: Set.set HS.rid) : GTot loc =
+  let Loc regions addrs aux_addrs aux = l in
+  Loc (Ghost.hide (Set.intersect (Ghost.reveal regions) rs))
     (fun r -> addrs r)
     (fun r -> aux_addrs r)
     (fun r n -> aux r n)
 
-let regions_of_loc_restrict_to_regions
-  (l: loc)
-  (rs: Set.set HS.rid)
-: Lemma
-  (regions_of_loc (restrict_to_regions l rs) == Set.intersect (regions_of_loc l) rs)
-  [SMTPat (regions_of_loc (restrict_to_regions l rs))]
-= assert (Set.equal (regions_of_loc (restrict_to_regions l rs)) (Set.intersect (regions_of_loc l) rs))
+let regions_of_loc_restrict_to_regions (l: loc) (rs: Set.set HS.rid)
+  : Lemma (regions_of_loc (restrict_to_regions l rs) == Set.intersect (regions_of_loc l) rs)
+    [SMTPat (regions_of_loc (restrict_to_regions l rs))] =
+  assert (Set.equal (regions_of_loc (restrict_to_regions l rs))
+        (Set.intersect (regions_of_loc l) rs))
 
-let addrs_of_loc_weak_restrict_to_regions
-  (l: loc)
-  (rs: Set.set HS.rid)
-  (r: HS.rid)
-: Lemma
-  (addrs_of_loc_weak (restrict_to_regions l rs) r == (if Set.mem r rs then addrs_of_loc_weak l r else Set.empty))
-  [SMTPat (addrs_of_loc_weak (restrict_to_regions l rs) r)]
-= assert (Set.equal (addrs_of_loc_weak (restrict_to_regions l rs) r) (if Set.mem r rs then addrs_of_loc_weak l r else Set.empty))
+let addrs_of_loc_weak_restrict_to_regions (l: loc) (rs: Set.set HS.rid) (r: HS.rid)
+  : Lemma
+    (addrs_of_loc_weak (restrict_to_regions l rs) r ==
+      (if Set.mem r rs then addrs_of_loc_weak l r else Set.empty))
+    [SMTPat (addrs_of_loc_weak (restrict_to_regions l rs) r)] =
+  assert (Set.equal (addrs_of_loc_weak (restrict_to_regions l rs) r)
+        (if Set.mem r rs then addrs_of_loc_weak l r else Set.empty))
 
-let addrs_of_loc_restrict_to_regions
-  (l: loc)
-  (rs: Set.set HS.rid)
-  (r: HS.rid)
-: Lemma
-  (addrs_of_loc (restrict_to_regions l rs) r == (if Set.mem r rs then addrs_of_loc l r else Set.empty))
-  [SMTPat (addrs_of_loc (restrict_to_regions l rs) r)]
-= assert (Set.equal (addrs_of_loc (restrict_to_regions l rs) r) (if Set.mem r rs then addrs_of_loc l r else Set.empty))
+let addrs_of_loc_restrict_to_regions (l: loc) (rs: Set.set HS.rid) (r: HS.rid)
+  : Lemma
+    (addrs_of_loc (restrict_to_regions l rs) r ==
+      (if Set.mem r rs then addrs_of_loc l r else Set.empty))
+    [SMTPat (addrs_of_loc (restrict_to_regions l rs) r)] =
+  assert (Set.equal (addrs_of_loc (restrict_to_regions l rs) r)
+        (if Set.mem r rs then addrs_of_loc l r else Set.empty))
 
-let loc_includes_restrict_to_regions
-  (l: loc)
-  (rs: Set.set HS.rid)
-: Lemma
-  (loc_includes l (restrict_to_regions l rs))
-= Classical.forall_intro loc_aux_includes_refl
+let loc_includes_restrict_to_regions (l: loc) (rs: Set.set HS.rid)
+  : Lemma (loc_includes l (restrict_to_regions l rs)) = Classical.forall_intro loc_aux_includes_refl
 
 #set-options "--z3rlimit 32"
 
-let loc_includes_loc_union_restrict_to_regions
-  (l: loc)
-  (rs: Set.set HS.rid)
-: Lemma
-  (loc_includes (loc_union (restrict_to_regions l rs) (restrict_to_regions l (Set.complement rs))) l)
-= Classical.forall_intro loc_aux_includes_refl
+let loc_includes_loc_union_restrict_to_regions (l: loc) (rs: Set.set HS.rid)
+  : Lemma
+  (loc_includes (loc_union (restrict_to_regions l rs) (restrict_to_regions l (Set.complement rs))) l
+  ) = Classical.forall_intro loc_aux_includes_refl
 
 #reset-options
 
-let loc_includes_loc_regions_restrict_to_regions
-  (l: loc)
-  (rs: Set.set HS.rid)
-: Lemma
-  (loc_includes (loc_regions rs) (restrict_to_regions l rs))
-= Classical.forall_intro loc_aux_includes_refl
+let loc_includes_loc_regions_restrict_to_regions (l: loc) (rs: Set.set HS.rid)
+  : Lemma (loc_includes (loc_regions rs) (restrict_to_regions l rs)) =
+  Classical.forall_intro loc_aux_includes_refl
 
 let modifies_only_live_regions rs l h h' =
   let s = l in
@@ -807,19 +590,15 @@ let modifies_loc_regions_intro rs h1 h2 = ()
 #set-options "--z3rlimit 16"
 
 let modifies_loc_addresses_intro_weak
-  (r: HS.rid)
-  (s: Set.set nat)
-  (l: loc)
-  (h1 h2: HS.mem)
-: Lemma
-  (requires (
-    HS.live_region h2 r /\
-    modifies (loc_union (loc_region_only r) l) h1 h2 /\
-    HS.modifies_ref r s h1 h2 /\
-    loc_disjoint l (loc_region_only r)
-  ))
-  (ensures (modifies (loc_union (loc_addresses r s) l) h1 h2))
-= assert (forall (t: Type) (pre: Preorder.preorder t) (p: HS.mreference t pre) . (HS.frameOf p == r /\ HS.contains h1 p /\ ~ (Set.mem (HS.as_addr p) s)) ==> (HS.contains h2 p /\ HS.sel h2 p == HS.sel h1 p));
+  (r: HS.rid) (s: Set.set nat) (l: loc) (h1: HS.mem) (h2: HS.mem)
+  : Lemma
+    (requires
+      (HS.live_region h2 r /\ modifies (loc_union (loc_region_only r) l) h1 h2 /\
+        HS.modifies_ref r s h1 h2 /\ loc_disjoint l (loc_region_only r)))
+    (ensures (modifies (loc_union (loc_addresses r s) l) h1 h2)) =
+  assert (forall (t: Type) (pre: Preorder.preorder t) (p: HS.mreference t pre).
+        (HS.frameOf p == r /\ HS.contains h1 p /\ ~(Set.mem (HS.as_addr p) s)) ==>
+        (HS.contains h2 p /\ HS.sel h2 p == HS.sel h1 p));
   assert (modifies_preserves_mreferences (loc_union (loc_addresses r s) l) h1 h2);
   assert (modifies_preserves_buffers (loc_union (loc_addresses r s) l) h1 h2)
 
@@ -830,8 +609,16 @@ let modifies_loc_addresses_intro_weak
 let modifies_loc_addresses_intro r s l h1 h2 =
   loc_includes_loc_regions_restrict_to_regions l (Set.singleton r);
   loc_includes_loc_union_restrict_to_regions l (Set.singleton r);
-  assert (modifies (loc_union (loc_region_only r) (loc_union (restrict_to_regions l (Set.singleton r)) (restrict_to_regions l (Set.complement (Set.singleton r))))) h1 h2);
-  modifies_loc_addresses_intro_weak r s (restrict_to_regions l (Set.complement (Set.singleton r))) h1 h2;
+  assert (modifies (loc_union (loc_region_only r)
+            (loc_union (restrict_to_regions l (Set.singleton r))
+                (restrict_to_regions l (Set.complement (Set.singleton r)))))
+        h1
+        h2);
+  modifies_loc_addresses_intro_weak r
+    s
+    (restrict_to_regions l (Set.complement (Set.singleton r)))
+    h1
+    h2;
   loc_includes_restrict_to_regions l (Set.complement (Set.singleton r))
 
 #reset-options
@@ -846,19 +633,15 @@ let modifies_none_modifies h1 h2 = ()
 
 let modifies_buffer_none_modifies h1 h2 = ()
 
-let modifies_0_modifies h1 h2 =
-  B.lemma_reveal_modifies_0 h1 h2
+let modifies_0_modifies h1 h2 = B.lemma_reveal_modifies_0 h1 h2
 
-let modifies_1_modifies #a b h1 h2 =
-  B.lemma_reveal_modifies_1 b h1 h2
+let modifies_1_modifies #a b h1 h2 = B.lemma_reveal_modifies_1 b h1 h2
 
-let modifies_2_modifies #a1 #a2 b1 b2 h1 h2 =
-  B.lemma_reveal_modifies_2 b1 b2 h1 h2
+let modifies_2_modifies #a1 #a2 b1 b2 h1 h2 = B.lemma_reveal_modifies_2 b1 b2 h1 h2
 
 #set-options "--z3rlimit 32"
 
-let modifies_3_modifies #a1 #a2 #a3 b1 b2 b3 h1 h2 =
-  B.lemma_reveal_modifies_3 b1 b2 b3 h1 h2
+let modifies_3_modifies #a1 #a2 #a3 b1 b2 b3 h1 h2 = B.lemma_reveal_modifies_3 b1 b2 b3 h1 h2
 
 #reset-options
 
@@ -868,9 +651,9 @@ let mreference_live_buffer_unused_in_disjoint #t1 #pre #t2 h b1 b2 = ()
 
 let buffer_live_mreference_unused_in_disjoint #t1 #t2 #pre h b1 b2 = ()
 
-
 let does_not_contain_addr' (h: HS.mem) (ra: HS.rid * nat) : GTot Type0 =
-  forall (a: Type) (rel: Preorder.preorder a) (r: HS.mreference a rel) . {:pattern (h `HS.contains` r) } (HS.frameOf r == fst ra /\ HS.as_addr r == snd ra /\ h `HS.contains` r) ==> False
+  forall (a: Type) (rel: Preorder.preorder a) (r: HS.mreference a rel). {:pattern (HS.contains h r)}
+    (HS.frameOf r == fst ra /\ HS.as_addr r == snd ra /\ HS.contains h r) ==> False
 
 let does_not_contain_addr = does_not_contain_addr'
 
@@ -886,98 +669,72 @@ let does_not_contain_addr_elim #a #rel r m x = ()
 
 #set-options "--z3rlimit 16"
 
-let modifies_only_live_addresses_weak
-  (r: HS.rid)
-  (a: Set.set nat)
-  (l: loc)
-  (h h' : HS.mem)
-: Lemma
-  (requires (
-    modifies (loc_union (loc_addresses r a) l) h h' /\
-    loc_disjoint (loc_addresses r a) l /\
-    (forall x . Set.mem x a ==> h `does_not_contain_addr` (r, x))
-  ))
-  (ensures (modifies l h h'))
-= assert (modifies_preserves_mreferences l h h')
+let modifies_only_live_addresses_weak (r: HS.rid) (a: Set.set nat) (l: loc) (h: HS.mem) (h': HS.mem)
+  : Lemma
+    (requires
+      (modifies (loc_union (loc_addresses r a) l) h h' /\ loc_disjoint (loc_addresses r a) l /\
+        (forall x. Set.mem x a ==> does_not_contain_addr h (r, x)))) (ensures (modifies l h h')) =
+  assert (modifies_preserves_mreferences l h h')
 
 #reset-options
 
 (* Restrict a set of locations along a set of addresses in a given region *)
 
-let restrict_to_addresses
-  (l: loc)
-  (r: HS.rid)
-  (as: Set.set nat)
-: Ghost loc
-  (requires (loc_region_only r `loc_includes` l))
-  (ensures (fun _ -> True))
-= let (Loc regions addrs aux_addrs aux) = l in
-  let aux_addrs' = if Set.mem r (Ghost.reveal regions) then Set.intersect (aux_addrs r) as else Set.empty in
-    Loc
-      (Ghost.hide (Set.intersect (Ghost.reveal regions) (Set.singleton r)))
-      (fun _ -> if Set.mem r (Ghost.reveal regions) then Set.intersect (addrs r) as else Set.empty)
-      (fun _ -> aux_addrs')
-      (fun r n -> aux r n)
+let restrict_to_addresses (l: loc) (r: HS.rid) (as: Set.set nat)
+  : Ghost loc (requires (loc_includes (loc_region_only r) l)) (ensures (fun _ -> True)) =
+  let Loc regions addrs aux_addrs aux = l in
+  let aux_addrs' =
+    if Set.mem r (Ghost.reveal regions) then Set.intersect (aux_addrs r) as else Set.empty
+  in
+  Loc (Ghost.hide (Set.intersect (Ghost.reveal regions) (Set.singleton r)))
+    (fun _ -> if Set.mem r (Ghost.reveal regions) then Set.intersect (addrs r) as else Set.empty)
+    (fun _ -> aux_addrs')
+    (fun r n -> aux r n)
 
-let regions_of_loc_restrict_to_addresses
-  (l: loc)
-  (r: HS.rid)
-  (as: Set.set nat)
-: Lemma
-  (requires (loc_region_only r `loc_includes` l))
-  (ensures (regions_of_loc (restrict_to_addresses l r as) == Set.intersect (regions_of_loc l) (Set.singleton r)))
-  [SMTPat (regions_of_loc (restrict_to_addresses l r as))]
-= assert (regions_of_loc (restrict_to_addresses l r as) `Set.equal` Set.intersect (regions_of_loc l) (Set.singleton r))
+let regions_of_loc_restrict_to_addresses (l: loc) (r: HS.rid) (as: Set.set nat)
+  : Lemma (requires (loc_includes (loc_region_only r) l))
+    (ensures
+      (regions_of_loc (restrict_to_addresses l r as) ==
+        Set.intersect (regions_of_loc l) (Set.singleton r)))
+    [SMTPat (regions_of_loc (restrict_to_addresses l r as))] =
+  assert (Set.equal (regions_of_loc (restrict_to_addresses l r as))
+        (Set.intersect (regions_of_loc l) (Set.singleton r)))
 
-let addrs_of_loc_weak_restrict_to_addresses
-  (l: loc)
-  (r: HS.rid)
-  (as: Set.set nat)
-  (r' : HS.rid)
-: Lemma
-  (requires (loc_region_only r `loc_includes` l))
-  (ensures (addrs_of_loc_weak (restrict_to_addresses l r as) r' == (if r = r' then Set.intersect (addrs_of_loc_weak l r) as else Set.empty)))
-  [SMTPat (addrs_of_loc_weak (restrict_to_addresses l r as) r')]
-= assert (addrs_of_loc_weak (restrict_to_addresses l r as) r `Set.equal` Set.intersect (addrs_of_loc_weak l r) as)
+let addrs_of_loc_weak_restrict_to_addresses (l: loc) (r: HS.rid) (as: Set.set nat) (r': HS.rid)
+  : Lemma (requires (loc_includes (loc_region_only r) l))
+    (ensures
+      (addrs_of_loc_weak (restrict_to_addresses l r as) r' ==
+        (if r = r' then Set.intersect (addrs_of_loc_weak l r) as else Set.empty)))
+    [SMTPat (addrs_of_loc_weak (restrict_to_addresses l r as) r')] =
+  assert (Set.equal (addrs_of_loc_weak (restrict_to_addresses l r as) r)
+        (Set.intersect (addrs_of_loc_weak l r) as))
 
-let addrs_of_loc_restrict_to_addresses
-  (l: loc)
-  (r: HS.rid)
-  (as: Set.set nat)
-  (r' : HS.rid)
-: Lemma
-  (requires (loc_region_only r `loc_includes` l))
-  (ensures (addrs_of_loc (restrict_to_addresses l r as) r' == (if r = r' then Set.intersect (addrs_of_loc l r) as else Set.empty)))
-  [SMTPat (addrs_of_loc (restrict_to_addresses l r as) r')]
-= assert (addrs_of_loc (restrict_to_addresses l r as) r `Set.equal` Set.intersect (addrs_of_loc l r) as);
-  assert (r <> r' ==> addrs_of_loc (restrict_to_addresses l r as) r' `Set.equal` Set.empty)
+let addrs_of_loc_restrict_to_addresses (l: loc) (r: HS.rid) (as: Set.set nat) (r': HS.rid)
+  : Lemma (requires (loc_includes (loc_region_only r) l))
+    (ensures
+      (addrs_of_loc (restrict_to_addresses l r as) r' ==
+        (if r = r' then Set.intersect (addrs_of_loc l r) as else Set.empty)))
+    [SMTPat (addrs_of_loc (restrict_to_addresses l r as) r')] =
+  assert (Set.equal (addrs_of_loc (restrict_to_addresses l r as) r)
+        (Set.intersect (addrs_of_loc l r) as));
+  assert (r <> r' ==> Set.equal (addrs_of_loc (restrict_to_addresses l r as) r') Set.empty)
 
-let loc_includes_restrict_to_addresses
-  (l: loc)
-  (r: HS.rid)
-  (as: Set.set nat)
-: Lemma
-  (requires (loc_region_only r `loc_includes` l))
-  (ensures (loc_includes l (restrict_to_addresses l r as)))
-= Classical.forall_intro loc_aux_includes_refl
+let loc_includes_restrict_to_addresses (l: loc) (r: HS.rid) (as: Set.set nat)
+  : Lemma (requires (loc_includes (loc_region_only r) l))
+    (ensures (loc_includes l (restrict_to_addresses l r as))) =
+  Classical.forall_intro loc_aux_includes_refl
 
-let loc_includes_loc_union_restrict_to_addresses
-  (l: loc)
-  (r: HS.rid)
-  (as: Set.set nat)
-: Lemma
-  (requires (loc_region_only r `loc_includes` l))
-  (ensures (loc_includes (loc_union (restrict_to_addresses l r as) (restrict_to_addresses l r (Set.complement as))) l))
-= Classical.forall_intro loc_aux_includes_refl
+let loc_includes_loc_union_restrict_to_addresses (l: loc) (r: HS.rid) (as: Set.set nat)
+  : Lemma (requires (loc_includes (loc_region_only r) l))
+    (ensures
+      (loc_includes (loc_union (restrict_to_addresses l r as)
+              (restrict_to_addresses l r (Set.complement as)))
+          l)) = Classical.forall_intro loc_aux_includes_refl
 
-let loc_includes_loc_addresses_restrict_to_addresses
-  (l: loc)
-  (r: HS.rid)
-  (as: Set.set nat)
-: Lemma
-  (requires (loc_region_only r `loc_includes` l))
-  (ensures (loc_includes (loc_addresses r as) (restrict_to_addresses l r as)))
-= Classical.forall_intro loc_aux_includes_refl
+let loc_includes_loc_addresses_restrict_to_addresses (l: loc) (r: HS.rid) (as: Set.set nat)
+  : Lemma (requires (loc_includes (loc_region_only r) l))
+    (ensures (loc_includes (loc_addresses r as) (restrict_to_addresses l r as))) =
+  Classical.forall_intro loc_aux_includes_refl
 
 #set-options "--z3rlimit 64"
 
@@ -994,10 +751,14 @@ let modifies_only_live_addresses r a l h h' =
   loc_includes_trans (loc_union (loc_union l_a l_r_not_a) l_not_r) (loc_union l_r l_not_r) l;
   loc_includes_trans (loc_union l_a l_not_a) (loc_union (loc_union l_a l_r_not_a) l_not_r) l;
   loc_includes_trans l' (loc_union l_a l_not_a) l;
-  modifies_loc_includes (loc_union (loc_addresses r a) l_not_a) h h' (loc_union (loc_addresses r a) l);
+  modifies_loc_includes (loc_union (loc_addresses r a) l_not_a)
+    h
+    h'
+    (loc_union (loc_addresses r a) l);
   modifies_only_live_addresses_weak r a l_not_a h h';
   loc_includes_restrict_to_regions l (Set.complement (Set.singleton r));
   loc_includes_restrict_to_addresses l_r r (Set.complement a);
   modifies_loc_includes l h h' l_not_a
 
 #reset-options
+
