ulib/FStar.Pervasives.Native.fst
@@ -1,84 +1,50 @@
 module FStar.Pervasives.Native
 open Prims
 
-type option (a:Type) =
+type option (a: Type) =
   | None : option a
-  | Some : v:a -> option a
+  | Some : v: a -> option a
 
 (* 'a * 'b *)
-type tuple2 'a 'b =
-  | Mktuple2: _1:'a -> _2:'b -> tuple2 'a 'b
+type tuple2 'a 'b = | Mktuple2 : _1: 'a -> _2: 'b -> tuple2 'a 'b
 
-let fst (x:tuple2 'a 'b) :'a = Mktuple2?._1 x
+let fst (x: tuple2 'a 'b) : 'a = Mktuple2?._1 x
 
-let snd (x:tuple2 'a 'b) :'b = Mktuple2?._2 x
+let snd (x: tuple2 'a 'b) : 'b = Mktuple2?._2 x
 
 (* 'a * 'b * 'c *)
-type tuple3 'a 'b 'c =
-  | Mktuple3: _1:'a
-           -> _2:'b
-           -> _3:'c
-          -> tuple3 'a 'b 'c
+type tuple3 'a 'b 'c = | Mktuple3 : _1: 'a -> _2: 'b -> _3: 'c -> tuple3 'a 'b 'c
 
 (* 'a * 'b * 'c * 'd *)
-type tuple4 'a 'b 'c 'd =
-  | Mktuple4: _1:'a
-           -> _2:'b
-           -> _3:'c
-           -> _4:'d
-           -> tuple4 'a 'b 'c 'd
+type tuple4 'a 'b 'c 'd = | Mktuple4 : _1: 'a -> _2: 'b -> _3: 'c -> _4: 'd -> tuple4 'a 'b 'c 'd
 
 (* 'a * 'b * 'c * 'd * 'e *)
 type tuple5 'a 'b 'c 'd 'e =
-  | Mktuple5: _1:'a
-           -> _2:'b
-           -> _3:'c
-           -> _4:'d
-           -> _5:'e
-           -> tuple5 'a 'b 'c 'd 'e
+  | Mktuple5 : _1: 'a -> _2: 'b -> _3: 'c -> _4: 'd -> _5: 'e -> tuple5 'a 'b 'c 'd 'e
 
 (* 'a * 'b * 'c * 'd * 'e * 'f *)
 type tuple6 'a 'b 'c 'd 'e 'f =
-  | Mktuple6: _1:'a
-           -> _2:'b
-           -> _3:'c
-           -> _4:'d
-           -> _5:'e
-           -> _6:'f
-           -> tuple6 'a 'b 'c 'd 'e 'f
+  | Mktuple6 : _1: 'a -> _2: 'b -> _3: 'c -> _4: 'd -> _5: 'e -> _6: 'f -> tuple6 'a 'b 'c 'd 'e 'f
 
 (* 'a * 'b * 'c * 'd * 'e * 'f * 'g *)
 type tuple7 'a 'b 'c 'd 'e 'f 'g =
-  | Mktuple7: _1:'a
-           -> _2:'b
-           -> _3:'c
-           -> _4:'d
-           -> _5:'e
-           -> _6:'f
-           -> _7:'g
-           -> tuple7 'a 'b 'c 'd 'e 'f 'g
+  | Mktuple7 : _1: 'a -> _2: 'b -> _3: 'c -> _4: 'd -> _5: 'e -> _6: 'f -> _7: 'g ->
+    tuple7 'a 'b 'c 'd 'e 'f 'g
 
 (* 'a * 'b * 'c * 'd * 'e * 'f * 'g * 'h *)
 type tuple8 'a 'b 'c 'd 'e 'f 'g 'h =
-  | Mktuple8: _1:'a
-           -> _2:'b
-           -> _3:'c
-           -> _4:'d
-           -> _5:'e
-           -> _6:'f
-           -> _7:'g
-           -> _8:'h
-           -> tuple8 'a 'b 'c 'd 'e 'f 'g 'h
+  | Mktuple8 : _1: 'a -> _2: 'b -> _3: 'c -> _4: 'd -> _5: 'e -> _6: 'f -> _7: 'g -> _8: 'h ->
+    tuple8 'a 'b 'c 'd 'e 'f 'g 'h
 
-
-(*********************************************************************************)
 (* Marking terms for normalization *)
-(*********************************************************************************)
-abstract let normalize_term (#a:Type) (x:a) : a = x
-abstract let normalize (a:Type0) :Type0 = a
 
 abstract
-noeq type norm_step =
+let normalize_term (#a: Type) (x: a) : a = x
+abstract
+let normalize (a: Type0) : Type0 = a
+
+abstract noeq
+type norm_step =
   | Simpl
   | Weak
   | HNF
@@ -86,26 +52,40 @@ noeq type norm_step =
   | Delta
   | Zeta
   | Iota
-  | UnfoldOnly:list string -> norm_step // each string is a fully qualified name like `A.M.f`
-  | UnfoldFully:list string -> norm_step // idem
-  | UnfoldAttr:#t:Type0 -> a:t -> norm_step
+  // each string is a fully qualified name like `A.M.f`
+  | UnfoldOnly : list string -> norm_step
+  // idem
+  | UnfoldFully : list string -> norm_step
+  | UnfoldAttr : #t: Type0 -> a: t -> norm_step
 
 // Helpers, so we don't expose the actual inductive
-abstract let simplify : norm_step = Simpl
-abstract let weak     : norm_step = Weak
-abstract let hnf      : norm_step = HNF
-abstract let primops  : norm_step = Primops
-abstract let delta    : norm_step = Delta
-abstract let zeta     : norm_step = Zeta
-abstract let iota     : norm_step = Iota
-abstract let delta_only (s:list string) : norm_step = UnfoldOnly s
-abstract let delta_fully (s:list string) : norm_step = UnfoldFully s
-abstract let delta_attr (#t:Type)(a:t) : norm_step = UnfoldAttr a
+abstract
+let simplify: norm_step = Simpl
+abstract
+let weak: norm_step = Weak
+abstract
+let hnf: norm_step = HNF
+abstract
+let primops: norm_step = Primops
+abstract
+let delta: norm_step = Delta
+abstract
+let zeta: norm_step = Zeta
+abstract
+let iota: norm_step = Iota
+abstract
+let delta_only (s: list string) : norm_step = UnfoldOnly s
+abstract
+let delta_fully (s: list string) : norm_step = UnfoldFully s
+abstract
+let delta_attr (#t: Type) (a: t) : norm_step = UnfoldAttr a
 
 // Normalization marker
-abstract let norm (s:list norm_step) (#a:Type) (x:a) : a = x
+abstract
+let norm (s: list norm_step) (#a: Type) (x: a) : a = x
 
-abstract val assert_norm : p:Type -> Pure unit (requires (normalize p)) (ensures (fun _ -> p))
+abstract
+val assert_norm: p: Type -> Pure unit (requires (normalize p)) (ensures (fun _ -> p))
 let assert_norm p = ()
 
 let normalize_term_spec (#a: Type) (x: a) : Lemma (normalize_term #a x == x) = ()
@@ -118,8 +98,8 @@ let norm_spec (s: list norm_step) (#a: Type) (x: a) : Lemma (norm s #a x == x) =
  * To circumvent this behavior, singleton can be used.
  * See the example usage in ulib/FStar.Algebra.Monoid.fst.
  *)
-irreducible let singleton (#a:Type) (x:a) :(y:a{y == x}) = x
-
+irreducible
+let singleton (#a: Type) (x: a) : (y: a{y == x}) = x
 
 (*
  * `with_type t e` is just an identity function, but it receives special treatment
@@ -127,4 +107,5 @@ irreducible let singleton (#a:Type) (x:a) :(y:a{y == x}) = x
  *  an SMT axiom:
  *  `forall t e.{:pattern (with_type t e)} has_type (with_type t e) t`
  *)
-let with_type (#t:Type) (e:t) = e
+let with_type (#t: Type) (e: t) = e
+
