ulib/FStar.Reflection.Data.fst
@@ -5,151 +5,132 @@ open FStar.Reflection.Types
 noeq
 type vconst =
   | C_Unit : vconst
-  | C_Int : int -> vconst // Not exposing the full details of our integer repr.
+  // Not exposing the full details of our integer repr.
+  | C_Int : int -> vconst
   | C_True : vconst
   | C_False : vconst
   | C_String : string -> vconst
-  (* TODO: complete *)
+(* TODO: complete *)
 
 // This is shadowing `pattern` from Prims (for smt_pats)
+
 noeq
 type pattern =
-    | Pat_Constant : vconst -> pattern              // A built-in constant
-    | Pat_Cons     : fv -> list pattern -> pattern  // A fully applied constructor
-    | Pat_Var      : bv -> pattern                  // Pattern bound variable
-    | Pat_Wild     : bv -> pattern                  // Wildcard (GM: why is this not Pat_var too?)
-    | Pat_Dot_Term : bv -> term -> pattern          // Dot pattern: resolved by other elements in the pattern and type
+  // A built-in constant
+  | Pat_Constant : vconst -> pattern
+  // A fully applied constructor
+  | Pat_Cons : fv -> list pattern -> pattern
+  // Pattern bound variable
+  | Pat_Var : bv -> pattern
+  // Wildcard (GM: why is this not Pat_var too?)
+  | Pat_Wild : bv -> pattern
+  // Dot pattern: resolved by other elements in the pattern and type
+  | Pat_Dot_Term : bv -> term -> pattern
 
-type branch = pattern * term  // | pattern -> term
+// | pattern -> term
+type branch = pattern * term
 
 type aqualv =
-    | Q_Implicit
-    | Q_Explicit
+  | Q_Implicit
+  | Q_Explicit
 
 type argv = term * aqualv
 
 noeq
-type bv_view = {
-    bv_ppname : string;
-    bv_index : int;
-    bv_sort : typ;
-}
+type bv_view = { bv_ppname:string; bv_index:int; bv_sort:typ }
 
 noeq
 type term_view =
-  | Tv_Var    : v:bv -> term_view
-  | Tv_BVar   : v:bv -> term_view
-  | Tv_FVar   : v:fv -> term_view
-  | Tv_App    : hd:term -> a:argv -> term_view
-  | Tv_Abs    : bv:binder -> body:term -> term_view
-  | Tv_Arrow  : bv:binder -> c:comp -> term_view
-  | Tv_Type   : unit -> term_view
-  | Tv_Refine : bv:bv -> ref:term -> term_view
-  | Tv_Const  : vconst -> term_view
-  | Tv_Uvar   : int -> typ -> term_view
-  | Tv_Let    : recf:bool -> bv:bv -> def:term -> body:term -> term_view
-  | Tv_Match  : scrutinee:term -> brs:(list branch) -> term_view
-  | Tv_AscribedT : e:term -> t:term -> tac:option term -> term_view
-  | Tv_AscribedC : e:term -> c:comp -> tac:option term -> term_view  
-  | Tv_Unknown  : term_view // Baked in "None"
+  | Tv_Var : v: bv -> term_view
+  | Tv_BVar : v: bv -> term_view
+  | Tv_FVar : v: fv -> term_view
+  | Tv_App : hd: term -> a: argv -> term_view
+  | Tv_Abs : bv: binder -> body: term -> term_view
+  | Tv_Arrow : bv: binder -> c: comp -> term_view
+  | Tv_Type : unit -> term_view
+  | Tv_Refine : bv: bv -> ref: term -> term_view
+  | Tv_Const : vconst -> term_view
+  | Tv_Uvar : int -> typ -> term_view
+  | Tv_Let : recf: bool -> bv: bv -> def: term -> body: term -> term_view
+  | Tv_Match : scrutinee: term -> brs: (list branch) -> term_view
+  | Tv_AscribedT : e: term -> t: term -> tac: option term -> term_view
+  | Tv_AscribedC : e: term -> c: comp -> tac: option term -> term_view
+  // Baked in "None"
+  | Tv_Unknown : term_view
 
 // Very basic for now
+
 noeq
 type comp_view =
-  | C_Total     : ret:typ -> decr:(option term) -> comp_view
-  | C_Lemma     : term -> term -> comp_view // pre & post
-  | C_Unknown   : comp_view
+  | C_Total : ret: typ -> decr: (option term) -> comp_view
+  // pre & post
+  | C_Lemma : term -> term -> comp_view
+  | C_Unknown : comp_view
 
 noeq
 type sigelt_view =
-  | Sg_Let :
-      (r:bool) ->
-      (fv:fv) ->
-      (typ:typ) ->
-      (def:term) ->
-      sigelt_view
-
+  | Sg_Let : r: bool -> fv: fv -> typ: typ -> def: term -> sigelt_view
   // Sg_Inductive basically coallesces the Sig_bundle used internally,
   // where the type definition and its constructors are split.
   // While that might be better for typechecking, this is probably better for metaprogrammers
   // (no mutually defined types for now)
-  | Sg_Inductive :
-      (nm:name) ->              // name of the inductive type being defined
-      (params:binders) ->       // parameters
-      (typ:typ) ->              // the type annotation for the inductive, i.e., indices -> Type #u
-      (cts:list name) ->        // constructor names
-      sigelt_view
-
-  | Sg_Constructor :
-      (name:name) ->
-      (typ:typ) ->
-      sigelt_view
-
+  // name of the inductive type being defined
+  | Sg_Inductive : 
+    nm: name ->
+    params:
+    // parameters
+    binders ->
+    typ:
+    // the type annotation for the inductive, i.e., indices -> Type #u
+    typ ->
+    cts:
+    // constructor names
+    list name ->
+    sigelt_view
+  | Sg_Constructor : name: name -> typ: typ -> sigelt_view
   | Unk
 
-let var : eqtype = nat
+let var: eqtype = nat
 
 type exp : Type =
   | Unit : exp
   | Var : var -> exp
   | Mult : exp -> exp -> exp
 
-
 type decls = list sigelt
 
-let rec forall_list (p:'a -> Type) (l:list 'a) : Type =
-    match l with
-    | [] -> True
-    | x::xs -> p x /\ forall_list p xs
+let rec forall_list (p: ('a -> Type)) (l: list 'a) : Type =
+  match l with
+  | [] -> True
+  | x :: xs -> p x /\ forall_list p xs
 
 (* Comparison of a term_view to term. Allows to recurse while changing the view *)
-val smaller : term_view -> term -> Type0
+val smaller: term_view -> term -> Type0
 let smaller tv t =
-    match tv with
-    | Tv_App l r ->
-        l << t /\ r << t /\ fst r << t
+  match tv with
+  | Tv_App l r -> l << t /\ r << t /\ fst r << t
+  | Tv_Abs b t' | Tv_Arrow b t' -> b << t /\ t' << t
+  | Tv_Refine b t' -> bv << t /\ t' << t
+  | Tv_Let r bv t1 t2 -> bv << t /\ t1 << t /\ t2 << t
+  | Tv_Match t1 brs -> t1 << t /\ (forall_list (fun (b, t') -> t' << t) brs)
+  | Tv_AscribedT e ty tac -> e << t /\ ty << t /\ tac << t
+  | Tv_AscribedC e c tac -> e << t /\ c << t /\ tac << t
+  | Tv_Type _ | Tv_Const _ | Tv_Unknown | Tv_Var _ | Tv_BVar _ | Tv_Uvar _ _ | Tv_FVar _ -> True
 
-    | Tv_Abs b t'
-    | Tv_Arrow b t' ->
-        b << t /\ t' << t
-
-    | Tv_Refine b t' ->
-        bv << t /\ t' << t
-
-    | Tv_Let r bv t1 t2 ->
-        bv << t /\ t1 << t /\ t2 << t
-
-    | Tv_Match t1 brs ->
-        t1 << t /\ (forall_list (fun (b, t') -> t' << t) brs)
-
-    | Tv_AscribedT e ty tac ->
-      e << t /\ ty << t /\ tac << t
-
-    | Tv_AscribedC e c tac ->
-      e << t /\ c << t /\ tac << t
-
-    | Tv_Type _
-    | Tv_Const _
-    | Tv_Unknown
-    | Tv_Var _
-    | Tv_BVar _
-    | Tv_Uvar _ _
-    | Tv_FVar _ -> True
-
-val smaller_comp : comp_view -> comp -> Type0
+val smaller_comp: comp_view -> comp -> Type0
 let smaller_comp cv c =
-    match cv with
-    | C_Total t md ->
-        t << c /\ (match md with | Some d -> d << c | None -> True)
-    | C_Lemma pre post ->
-        pre << c /\ post << c
-    | C_Unknown ->
-        True
+  match cv with
+  | C_Total t md ->
+    t << c /\
+    (match md with
+      | Some d -> d << c
+      | None -> True)
+  | C_Lemma pre post -> pre << c /\ post << c
+  | C_Unknown -> True
 
-val smaller_bv : bv_view -> bv -> Type0
-let smaller_bv bvv bv =
-    bvv.bv_sort << bv
+val smaller_bv: bv_view -> bv -> Type0
+let smaller_bv bvv bv = bvv.bv_sort << bv
 
-val smaller_binder : binder -> (bv * aqualv) -> Type0
-let smaller_binder b (bv, _) =
-    bv << b
+val smaller_binder: binder -> (bv * aqualv) -> Type0
+let smaller_binder b (bv, _) = bv << b
+
