ulib/FStar.Tactics.Derived.fst
@@ -8,351 +8,329 @@ open FStar.Tactics.Builtins
 open FStar.Tactics.Util
 module L = FStar.List.Tot
 
+
 (** Set the guard policy only locally, without affecting calling code *)
-let with_policy pol (f : unit -> Tac 'a) : Tac 'a =
-    let old_pol = get_guard_policy () in
-    set_guard_policy pol;
-    let r = f () in
-    set_guard_policy old_pol;
-    r
+let with_policy pol (f: (unit -> Tac 'a)) : Tac 'a =
+  let old_pol = get_guard_policy () in
+  set_guard_policy pol;
+  let r = f () in
+  set_guard_policy old_pol;
+  r
+
 
 (** [exact e] will solve a goal [Gamma |- w : t] if [e] has type exactly
 [t] in [Gamma]. Also, [e] needs to unift with [w], but this will almost
 always be the case since [w] is usually a uvar. *)
-let exact (t : term) : Tac unit =
-    with_policy SMT (fun () -> t_exact false t)
+let exact (t: term) : Tac unit = with_policy SMT (fun () -> t_exact false t)
+
 
 (** Like [exact], but allows for the term [e] to have a type [t] only
 under some guard [g], adding the guard as a goal. *)
-let exact_guard (t : term) : Tac unit =
-    with_policy Goal (fun () -> t_exact false t)
+let exact_guard (t: term) : Tac unit = with_policy Goal (fun () -> t_exact false t)
 
-let cur_module () : Tac (list string) =
-    moduleof (cur_env ())
+let cur_module () : Tac (list string) = moduleof (cur_env ())
 
-let focus (f : unit -> Tac 'a) : Tac 'a =
-    let res, _ = divide 1 f (fun () -> ()) in
-    res
+let focus (f: (unit -> Tac 'a)) : Tac 'a =
+  let res, _ = divide 1 f (fun () -> ()) in
+  res
 
-let rec repeatn (#a:Type) (n : int) (t : unit -> Tac a) : Tac (list a) =
-    if n = 0
-    then []
-    else let x = t () in
-         let xs = repeatn (n - 1) t in
-         x :: xs
+let rec repeatn (#a: Type) (n: int) (t: (unit -> Tac a)) : Tac (list a) =
+  if n = 0
+  then []
+  else
+    let x = t () in
+    let xs = repeatn (n - 1) t in
+    x :: xs
 
-let fresh_uvar (o : option typ) : Tac term =
-    let e = cur_env () in
-    uvar_env e o
+let fresh_uvar (o: option typ) : Tac term =
+  let e = cur_env () in
+  uvar_env e o
 
-let exact_args (qs : list aqualv) (t : term) : Tac unit =
-    focus (fun () ->
+let exact_args (qs: list aqualv) (t: term) : Tac unit =
+  focus (fun () ->
         let n = List.length qs in
         let uvs = repeatn n (fun () -> fresh_uvar None) in
         let t' = mk_app t (zip uvs qs) in
         exact t';
-        iter (fun uv -> if is_uvar uv
-                        then unshelve uv
-                        else ()) (L.rev uvs)
-    )
+        iter (fun uv -> if is_uvar uv then unshelve uv) (L.rev uvs))
 
-let exact_n (n : int) (t : term) : Tac unit =
-    exact_args (repeatn n (fun () -> Q_Explicit)) t
+let exact_n (n: int) (t: term) : Tac unit = exact_args (repeatn n (fun () -> Q_Explicit)) t
 
 let fresh_bv t =
-    (* These bvs are fresh anyway through a separate counter,
+  (* These bvs are fresh anyway through a separate counter,
      * but adding the integer allows for more readable code when
      * generating code *)
-    let i = fresh () in
-    fresh_bv_named ("x" ^ string_of_int i) t
+  let i = fresh () in
+  fresh_bv_named ("x" ^ string_of_int i) t
 
-let fresh_binder_named nm t =
-    mk_binder (fresh_bv_named nm t)
+let fresh_binder_named nm t = mk_binder (fresh_bv_named nm t)
 
 let fresh_binder t =
-    (* See comment in fresh_bv *)
-    let i = fresh () in
-    fresh_binder_named ("x" ^ string_of_int i) t
+  (* See comment in fresh_bv *)
+  let i = fresh () in
+  fresh_binder_named ("x" ^ string_of_int i) t
 
-let norm_term (s : list norm_step) (t : term) : Tac term =
-    let e = cur_env () in
-    norm_term_env e s t
+let norm_term (s: list norm_step) (t: term) : Tac term =
+  let e = cur_env () in
+  norm_term_env e s t
 
 let idtac () : Tac unit = ()
 
-let guard (b : bool) : Tac unit =
-    if b
-    then ()
-    else fail "guard failed"
+let guard (b: bool) : Tac unit = if b then () else fail "guard failed"
 
-let or_else (#a:Type) (t1 : unit -> Tac a) (t2 : unit -> Tac a) : Tac a =
-    match trytac t1 with
-    | Some x -> x
-    | None -> t2 ()
+let or_else (#a: Type) (t1: (unit -> Tac a)) (t2: (unit -> Tac a)) : Tac a =
+  match trytac t1 with
+  | Some x -> x
+  | None -> t2 ()
 
-let rec first (ts : list (unit -> Tac 'a)) : Tac 'a =
-    match ts with
-    | [] -> fail "no tactics to try"
-    | [t] -> t ()
-    | t::ts -> or_else t (fun () -> first ts)
+let rec first (ts: list (unit -> Tac 'a)) : Tac 'a =
+  match ts with
+  | [] -> fail "no tactics to try"
+  | [t] -> t ()
+  | t :: ts -> or_else t (fun () -> first ts)
 
-let rec repeat (#a:Type) (t : unit -> Tac a) : Tac (list a) =
-    match trytac t with
-    | None -> []
-    | Some x -> let xs = repeat t in x::xs
+let rec repeat (#a: Type) (t: (unit -> Tac a)) : Tac (list a) =
+  match trytac t with
+  | None -> []
+  | Some x ->
+    let xs = repeat t in
+    x :: xs
 
-let repeat1 (#a:Type) (t : unit -> Tac a) : Tac (list a) =
-    let x = t () in
-    x :: repeat t
+let repeat1 (#a: Type) (t: (unit -> Tac a)) : Tac (list a) =
+  let x = t () in
+  x :: repeat t
 
-
-let discard (tau : unit -> Tac 'a) : unit -> Tac unit =
-    fun () -> let _ = tau () in ()
+let discard (tau: (unit -> Tac 'a)) : unit -> Tac unit =
+  fun () ->
+    let _ = tau () in
+    ()
 
 // TODO: do we want some value of this?
-let rec repeatseq (#a:Type) (t : unit -> Tac a) : Tac unit =
-    let _ = trytac (fun () -> (discard t) `seq` (discard (fun () -> repeatseq t))) in ()
+let rec repeatseq (#a: Type) (t: (unit -> Tac a)) : Tac unit =
+  let _ = trytac (fun () -> seq (discard t) (discard (fun () -> repeatseq t))) in
+  ()
 
-let admit1 () : Tac unit =
-    tadmit ()
+let admit1 () : Tac unit = tadmit ()
 
 let admit_all () : Tac unit =
-    let _ = repeat tadmit in
-    ()
+  let _ = repeat tadmit in
+  ()
 
-let skip_guard () : Tac unit =
-    if is_guard ()
-    then smt ()
-    else fail ""
+let skip_guard () : Tac unit = if is_guard () then smt () else fail ""
 
 let guards_to_smt () : Tac unit =
-    let _ = repeat skip_guard in
-    ()
+  let _ = repeat skip_guard in
+  ()
 
-let simpl   () : Tac unit = norm [simplify; primops]
-let whnf    () : Tac unit = norm [weak; hnf; primops]
+let simpl () : Tac unit = norm [simplify; primops]
+let whnf () : Tac unit = norm [weak; hnf; primops]
 let compute () : Tac unit = norm [primops; iota; delta; zeta]
 
 let intros () : Tac (list binder) = repeat intro
 
-private val __cut : (a:Type) -> (b:Type) -> (a -> b) -> a -> b
-private let __cut a b f x = f x
+private
+val __cut: a: Type -> b: Type -> (a -> b) -> a -> b
+private
+let __cut a b f x = f x
 
-let tcut (t:term) : Tac binder =
-    let g = cur_goal () in
-    let tt = mk_e_app (`__cut) [t; g] in
-    apply tt;
-    intro ()
+let tcut (t: term) : Tac binder =
+  let g = cur_goal () in
+  let tt = mk_e_app (`__cut) [t; g] in
+  apply tt;
+  intro ()
 
-let pose (t:term) : Tac binder =
-    apply (`__cut);
-    flip ();
-    exact t;
-    let _ = trytac flip in // maybe we have less than 2 goals now
-    intro ()
+let pose (t: term) : Tac binder =
+  apply (`__cut);
+  flip ();
+  exact t;
+  // maybe we have less than 2 goals now
+  let _ = trytac flip in
+  intro ()
 
-let intro_as (s:string) : Tac binder =
-    let b = intro () in
-    rename_to b s;
-    b
+let intro_as (s: string) : Tac binder =
+  let b = intro () in
+  rename_to b s;
+  b
 
-let pose_as (s:string) (t:term) : Tac binder =
-    let b = pose t in
-    rename_to b s;
-    b
+let pose_as (s: string) (t: term) : Tac binder =
+  let b = pose t in
+  rename_to b s;
+  b
 
-let rec revert_all (bs:binders) : Tac unit =
-    match bs with
-    | [] -> ()
-    | _::tl -> revert ();
-               revert_all tl
+let rec revert_all (bs: binders) : Tac unit =
+  match bs with
+  | [] -> ()
+  | _ :: tl -> revert (); revert_all tl
 
 // Cannot define this inside `assumption` due to #1091
+
 private
-let rec __assumption_aux (bs : binders) : Tac unit =
-    match bs with
-    | [] ->
-        fail "no assumption matches goal"
-    | b::bs ->
-        let t = pack_ln (Tv_Var (bv_of_binder b)) in
-        or_else (fun () -> exact t) (fun () -> __assumption_aux bs)
+let rec __assumption_aux (bs: binders) : Tac unit =
+  match bs with
+  | [] -> fail "no assumption matches goal"
+  | b :: bs ->
+    let t = pack_ln (Tv_Var (bv_of_binder b)) in
+    or_else (fun () -> exact t) (fun () -> __assumption_aux bs)
 
-let assumption () : Tac unit =
-    __assumption_aux (binders_of_env (cur_env ()))
+let assumption () : Tac unit = __assumption_aux (binders_of_env (cur_env ()))
 
-let destruct_equality_implication (t:term) : Tac (option (formula * term)) =
-    match term_as_formula t with
-    | Implies lhs rhs ->
-        let lhs = term_as_formula' lhs in
-        begin match lhs with
-        | Comp (Eq _) _ _ -> Some (lhs, rhs)
-        | _ -> None
-        end
-    | _ -> None
+let destruct_equality_implication (t: term) : Tac (option (formula * term)) =
+  match term_as_formula t with
+  | Implies lhs rhs ->
+    let lhs = term_as_formula' lhs in
+    (match lhs with
+      | Comp (Eq _) _ _ -> Some (lhs, rhs)
+      | _ -> None)
+  | _ -> None
 
-let rec try_rewrite_equality (x:term) (bs:binders) : Tac unit =
-    match bs with
-    | [] -> ()
-    | x_t::bs ->
-        begin match term_as_formula (type_of_binder x_t) with
-        | Comp (Eq _) y _ ->
-            if term_eq x y
-            then rewrite x_t
-            else try_rewrite_equality x bs
-        | _ ->
-            try_rewrite_equality x bs
-        end
+let rec try_rewrite_equality (x: term) (bs: binders) : Tac unit =
+  match bs with
+  | [] -> ()
+  | x_t :: bs ->
+    match term_as_formula (type_of_binder x_t) with
+    | Comp (Eq _) y _ -> if term_eq x y then rewrite x_t else try_rewrite_equality x bs
+    | _ -> try_rewrite_equality x bs
 
-let rec rewrite_all_context_equalities (bs:binders) : Tac unit =
-    match bs with
-    | [] -> ()
-    | x_t::bs -> begin
-        begin match term_as_formula (type_of_binder x_t) with
-        | Comp (Eq _) lhs _ ->
-            begin match inspect_ln lhs with
-            | Tv_Var _ -> rewrite x_t
-            | _ -> ()
-            end
-        | _ -> () end;
-        rewrite_all_context_equalities bs
-    end
+let rec rewrite_all_context_equalities (bs: binders) : Tac unit =
+  match bs with
+  | [] -> ()
+  | x_t :: bs ->
+    (match term_as_formula (type_of_binder x_t) with
+      | Comp (Eq _) lhs _ ->
+        (match inspect_ln lhs with
+          | Tv_Var _ -> rewrite x_t
+          | _ -> ())
+      | _ -> ());
+    rewrite_all_context_equalities bs
 
 let rewrite_eqs_from_context () : Tac unit =
-    rewrite_all_context_equalities (binders_of_env (cur_env ()))
+  rewrite_all_context_equalities (binders_of_env (cur_env ()))
 
-let rewrite_equality (t:term) : Tac unit =
-    try_rewrite_equality t (binders_of_env (cur_env ()))
+let rewrite_equality (t: term) : Tac unit = try_rewrite_equality t (binders_of_env (cur_env ()))
 
-let unfold_def (t:term) : Tac unit =
-    match inspect t with
-    | Tv_FVar fv ->
-        let n = String.concat "." (inspect_fv fv) in
-        norm [delta_fully [n]]
-    | _ -> fail "unfold_def: term is not a fv"
+let unfold_def (t: term) : Tac unit =
+  match inspect t with
+  | Tv_FVar fv ->
+    let n = String.concat "." (inspect_fv fv) in
+    norm [delta_fully [n]]
+  | _ -> fail "unfold_def: term is not a fv"
 
-let grewrite' (t1 t2 eq : term) : Tac unit =
-    let g = cur_goal () in
-    match term_as_formula g with
-    | Comp (Eq _) l _ ->
-        if term_eq l t1
-        then exact eq
-        else trefl ()
-    | _ ->
-        fail "impossible"
+let grewrite' (t1: term) (t2: term) (eq: term) : Tac unit =
+  let g = cur_goal () in
+  match term_as_formula g with
+  | Comp (Eq _) l _ -> if term_eq l t1 then exact eq else trefl ()
+  | _ -> fail "impossible"
 
-let mk_squash (t : term) : term =
-    let sq : term = pack_ln (Tv_FVar (pack_fv squash_qn)) in
-    mk_e_app sq [t]
+let mk_squash (t: term) : term =
+  let sq: term = pack_ln (Tv_FVar (pack_fv squash_qn)) in
+  mk_e_app sq [t]
 
-let mk_sq_eq (t1 t2 : term) : term =
-    let eq : term = pack_ln (Tv_FVar (pack_fv eq2_qn)) in
-    mk_squash (mk_e_app eq [t1; t2])
+let mk_sq_eq (t1: term) (t2: term) : term =
+  let eq: term = pack_ln (Tv_FVar (pack_fv eq2_qn)) in
+  mk_squash (mk_e_app eq [t1; t2])
 
-let grewrite (t1 t2 : term) : Tac unit =
-    let e = tcut (mk_sq_eq t1 t2) in
-    pointwise (fun () -> grewrite' t1 t2 (pack_ln (Tv_Var (bv_of_binder e))))
+let grewrite (t1: term) (t2: term) : Tac unit =
+  let e = tcut (mk_sq_eq t1 t2) in
+  pointwise (fun () -> grewrite' t1 t2 (pack_ln (Tv_Var (bv_of_binder e))))
 
+let rec iseq (ts: list (unit -> Tac unit)) : Tac unit =
+  match ts with
+  | t :: ts ->
+    let _ = divide 1 t (fun () -> iseq ts) in
+    ()
+  | [] -> ()
 
-
-let rec iseq (ts : list (unit -> Tac unit)) : Tac unit =
-    match ts with
-    | t::ts -> let _ = divide 1 t (fun () -> iseq ts) in ()
-    | []    -> ()
-
-private val __witness : (#a:Type) -> (x:a) -> (#p:(a -> Type)) -> squash (p x) -> squash (l_Exists p)
-private let __witness #a x #p _ =
-  let id (a:Type) = a in
-  let x : squash (exists x. id (p x)) = () in //an indirection to tickle the SMT encoding
+private
+val __witness: #a: Type -> x: a -> #p: (a -> Type) -> squash (p x) -> squash (l_Exists p)
+private
+let __witness #a x #p _ =
+  let id (a: Type) = a in
+  //an indirection to tickle the SMT encoding
+  let x: squash (exists x. id (p x)) = () in
   x
 
-let witness (t : term) : Tac unit =
-    apply_raw (`__witness);
-    exact t
+let witness (t: term) : Tac unit = apply_raw (`__witness); exact t
 
-private val push1 : (#p:Type) -> (#q:Type) ->
-                        squash (p ==> q) ->
-                        squash p ->
-                        squash q
-private let push1 #p #q f u = ()
+private
+val push1: #p: Type -> #q: Type -> squash (p ==> q) -> squash p -> squash q
+private
+let push1 #p #q f u = ()
 
 (*
  * Some easier applying, which should prevent frustation
  * (or cause more when it doesn't do what you wanted to)
  *)
-val apply_squash_or_lem : d:nat -> term -> Tac unit
+val apply_squash_or_lem: d: nat -> term -> Tac unit
 let rec apply_squash_or_lem d t =
-    // Fuel cutoff, just in case.
-    if d <= 0 then fail "mapply: out of fuel" else begin
+  // Fuel cutoff, just in case.
+  if d <= 0
+  then fail "mapply: out of fuel"
+  else
     let g = cur_goal () in
     let ty = tc t in
     let tys, c = collect_arr ty in
     match inspect_comp c with
     | C_Lemma pre post ->
-       begin
-       (* What I would really like to do here is unify `mk_squash post` and the goal,
+      (* What I would really like to do here is unify `mk_squash post` and the goal,
         * but it didn't work on a first try, so just doing this for now *)
-       match trytac (fun () -> apply_lemma t) with
-       | Some _ -> () // Success
-       | None ->
-           let post = norm_term [] post in
-           (* Is the lemma an implication? We can try to intro *)
-           match term_as_formula' post with
-           | Implies p q ->
-               apply (`push1);
-               apply_squash_or_lem (d-1) t
-
-           | _ ->
-               fail "mapply: can't apply (1)"
-       end
+      (match trytac (fun () -> apply_lemma t) with
+        | Some _ ->
+          // Success
+          ()
+        | None ->
+          let post = norm_term [] post in
+          (* Is the lemma an implication? We can try to intro *)
+          match term_as_formula' post with
+          | Implies p q -> apply (`push1); apply_squash_or_lem (d - 1) t
+          | _ -> fail "mapply: can't apply (1)")
     | C_Total rt _ ->
-       begin match unsquash rt with
-       (* If the function returns a squash, just apply it, since our goals are squashed *)
-       | Some _ -> apply_lemma t
-       (* If not, we can try to introduce the squash ourselves first *)
-       | None ->
-           apply (`FStar.Squash.return_squash);
-           apply t
-       end
+      (match unsquash rt with
+        | Some _ ->
+          (* If the function returns a squash, just apply it, since our goals are squashed *)
+          apply_lemma t
+        | None ->
+          (* If not, we can try to introduce the squash ourselves first *)
+          apply (`FStar.Squash.return_squash);
+          apply t)
     | _ -> fail "mapply: can't apply (2)"
-    end
 
 (* `m` is for `magic` *)
-let mapply (t : term) : Tac unit =
-    apply_squash_or_lem 10 t
+let mapply (t: term) : Tac unit = apply_squash_or_lem 10 t
 
 private
 let dump_admit () : Tac unit =
-  clear_top (); // gets rid of the unit binder
+  // gets rid of the unit binder
+  clear_top ();
   admit1 ()
 
-assume val admit_goal : #a:Type -> unit ->
-    Pure a (requires (by_tactic dump_admit a))
-           (ensures (fun _ -> False))
+assume
+val admit_goal: #a: Type -> unit ->
+  Pure a (requires (by_tactic dump_admit a)) (ensures (fun _ -> False))
 
-let change_with t1 t2 =
-    focus (fun () ->
-        grewrite t1 t2;
-        iseq [idtac; trivial]
-    )
+let change_with t1 t2 = focus (fun () -> grewrite t1 t2; iseq [idtac; trivial])
 
-private val conv : #x:Type -> #y:Type -> squash (y == x) -> x -> y
-private let conv #x #y eq w = w
+private
+val conv: #x: Type -> #y: Type -> squash (y == x) -> x -> y
+private
+let conv #x #y eq w = w
 
-let change_sq t1 =
-    change (mk_e_app (`squash) [t1])
+let change_sq t1 = change (mk_e_app (`squash) [t1])
 
-let finish_by (t : unit -> Tac 'a) : Tac 'a =
-    let x = t () in
-    or_else qed (fun () -> fail "finish_by: not finished");
-    x
+let finish_by (t: (unit -> Tac 'a)) : Tac 'a =
+  let x = t () in
+  or_else qed (fun () -> fail "finish_by: not finished");
+  x
 
-let solve_then #a #b (t1 : unit -> Tac a) (t2 : a -> Tac b) : Tac b =
-    dup ();
-    let x = focus (fun () -> finish_by t1) in
-    let y = t2 x in
-    trefl ();
-    y
+let solve_then #a #b (t1: (unit -> Tac a)) (t2: (a -> Tac b)) : Tac b =
+  dup ();
+  let x = focus (fun () -> finish_by t1) in
+  let y = t2 x in
+  trefl ();
+  y
 
 (* Some syntax utility functions *)
-let bv_to_term (bv : bv) : Tac term = pack (Tv_Var bv)
-let binder_to_term (b : binder) : Tac term = let bv, _ = inspect_binder b in bv_to_term bv
+let bv_to_term (bv: bv) : Tac term = pack (Tv_Var bv)
+let binder_to_term (b: binder) : Tac term =
+  let bv, _ = inspect_binder b in
+  bv_to_term bv
+
