ulib/FStar.Tactics.Effect.fst
@@ -6,26 +6,24 @@ open FStar.Tactics.Result
 (* This module is extracted, don't add any `assume val`s or extraction
  * will break. (`synth_by_tactic` is fine) *)
 
-let __tac (a:Type) = proofstate -> M (__result a)
+let __tac (a: Type) = proofstate -> M (__result a)
 
 (* monadic return *)
-val __ret : a:Type -> x:a -> __tac a
-let __ret a x = fun (s:proofstate) -> Success x s
+val __ret: a: Type -> x: a -> __tac a
+let __ret a x = fun (s: proofstate) -> Success x s
 
 (* monadic bind *)
-let __bind (a:Type) (b:Type) (r1 r2:range) (t1:__tac a) (t2:a -> __tac b) : __tac b =
-    fun ps ->
-        let ps = set_proofstate_range ps (FStar.Range.prims_to_fstar_range r1) in
-        let ps = incr_depth ps in
-        let r = t1 ps in
-        match r with
-        | Success a ps'  ->
-            let ps' = set_proofstate_range ps' (FStar.Range.prims_to_fstar_range r2) in
-            // Force evaluation of __tracepoint q
-            begin match tracepoint ps' with
-            | () -> t2 a (decr_depth ps')
-            end
-        | Failed msg ps' -> Failed msg ps'
+let __bind (a: Type) (b: Type) (r1: range) (r2: range) (t1: __tac a) (t2: (a -> __tac b)) : __tac b =
+  fun ps ->
+    let ps = set_proofstate_range ps (FStar.Range.prims_to_fstar_range r1) in
+    let ps = incr_depth ps in
+    let r = t1 ps in
+    match r with
+    | Success a ps' ->
+      let ps' = set_proofstate_range ps' (FStar.Range.prims_to_fstar_range r2) in
+      // Force evaluation of __tracepoint q
+      (match tracepoint ps' with | () -> t2 a (decr_depth ps'))
+    | Failed msg ps' -> Failed msg ps'
 
 (* Actions *)
 let __get () : __tac proofstate = fun s0 -> Success s0 s0
@@ -41,57 +39,72 @@ let __tac_wp a = proofstate -> (__result a -> Tot Type0) -> Tot Type0
  *
  * So, override `bind_wp` for the effect with an efficient one.
  *)
-unfold let g_bind (a:Type) (b:Type) (wp:__tac_wp a) (f:a -> __tac_wp b) = fun ps post ->
-    wp ps (fun m' -> match m' with
-                     | Success a q -> f a q post
-                     | Failed msg q -> post (Failed msg q))
-
-unfold let g_compact (a:Type) (wp:__tac_wp a) : __tac_wp a =
-    fun ps post -> forall k. (forall (r:__result a).{:pattern (guard_free (k r))} post r ==> k r) ==> wp ps k
-
-unfold let __TAC_eff_override_bind_wp (r:range) (a:Type) (b:Type) (wp:__tac_wp a) (f:a -> __tac_wp b) =
-    g_compact b (g_bind a b wp f)
-
-(* total  *) //disable the termination check, although it remains reifiable
-[@ dm4f_bind_range ]
-reifiable reflectable new_effect {
-  TAC : a:Type -> Effect
-  with repr     = __tac
-     ; bind     = __bind
-     ; return   = __ret
-     ; __get    = __get
-}
-effect Tac  (a:Type) = TAC a (fun i post -> forall j. post j)
-effect TacF (a:Type) = TAC a (fun _ _ -> False) // A variant that doesn't prove totality (nor type safety!)
+unfold
+let g_bind (a: Type) (b: Type) (wp: __tac_wp a) (f: (a -> __tac_wp b)) =
+  fun ps post ->
+    wp ps
+      (function
+        | Success a q -> f a q post
+        | Failed msg q -> post (Failed msg q))
 
 unfold
-let lift_div_tac (a:Type) (wp:pure_wp a) : __tac_wp a =
-    fun ps p -> wp (fun x -> p (Success x ps))
+let g_compact (a: Type) (wp: __tac_wp a) : __tac_wp a =
+  fun ps post ->
+    forall k. (forall (r: __result a). {:pattern (guard_free (k r))} post r ==> k r) ==> wp ps k
 
-sub_effect DIV ~> TAC = lift_div_tac
+unfold
+let __TAC_eff_override_bind_wp
+  (r: range) (a: Type) (b: Type) (wp: __tac_wp a) (f: (a -> __tac_wp b)) =
+  g_compact b (g_bind a b wp f)
+
+(* total  *)
+//disable the termination check, although it remains reifiable
+
+[@ dm4f_bind_range]
+reifiable reflectable
+new_effect {
+  TAC : a: Type -> Effect
+  with
+    repr = __tac
+  ; bind = __bind
+  ; return = __ret
+  ; __get = __get
+}
+effect Tac (a: Type) = TAC a (fun i post -> forall j. post j)
+// A variant that doesn't prove totality (nor type safety!)
+effect TacF (a: Type) = TAC a (fun _ _ -> False)
+
+unfold
+let lift_div_tac (a: Type) (wp: pure_wp a) : __tac_wp a = fun ps p -> wp (fun x -> p (Success x ps))
+
+sub_effect DIV ~> TAC { lift_wp = lift_div_tac }
 
 abstract
-let __by_tactic (t:__tac 'a) (p:Type) : Type = p
+let __by_tactic (t: __tac 'a) (p: Type) : Type = p
 
-unfold let by_tactic (t : unit -> Tac 'a) (p:Type) : Type = __by_tactic (reify (t ())) p
+unfold
+let by_tactic (t: (unit -> Tac 'a)) (p: Type) : Type = __by_tactic (reify (t ())) p
 
 // This will run the tactic in order to (try to) produce a term of type t
 // It should not lead to any inconsistency, as any time this term appears
 // during typechecking, it is forced to be fully applied and the tactic
 // is run. A failure of the tactic is a typechecking failure.
 // TODO: `a` is really fixed to unit for now. Make it consistent
-assume val synth_by_tactic : (#t:Type) -> (unit -> Tac unit) -> Tot t
+assume
+val synth_by_tactic: #t: Type -> (unit -> Tac unit) -> Tot t
 
-let assert_by_tactic (p:Type) (t:unit -> Tac unit)
-  : Pure unit
-         (requires (by_tactic t (squash p)))
-         (ensures (fun _ -> p))
-  = ()
+let assert_by_tactic (p: Type) (t: (unit -> Tac unit))
+  : Pure unit (requires (by_tactic t (squash p))) (ensures (fun _ -> p)) = ()
 
 (* We don't peel off all `by_tactic`s in negative positions, so give the SMT a way to reason about them *)
-val by_tactic_seman : a:Type -> tau:(unit -> Tac a) -> phi:Type -> Lemma (by_tactic tau phi ==> phi) [SMTPat (by_tactic tau phi)]
+val by_tactic_seman: a: Type -> tau: (unit -> Tac a) -> phi: Type ->
+  Lemma (by_tactic tau phi ==> phi) [SMTPat (by_tactic tau phi)]
 let by_tactic_seman a tau phi = ()
 
 // TcTerm needs these two names typecheck tactics against
-private let tactic a = unit -> TacF a // we don't care if the tactic is satisfiable before running it
-private let reify_tactic (t : tactic 'a) : __tac 'a = reify (t ())
+// we don't care if the tactic is satisfiable before running it
+private
+let tactic a = unit -> TacF a
+private
+let reify_tactic (t: tactic 'a) : __tac 'a = reify (t ())
+
