ulib/FStar.Tactics.Logic.fst
@@ -6,165 +6,171 @@ open FStar.Tactics.Derived
 open FStar.Reflection
 open FStar.Reflection.Formula
 
-private val revert_squash : (#a:Type) -> (#b : (a -> Type)) ->
-                            (squash (forall (x:a). b x)) ->
-                            x:a -> squash (b x)
-let revert_squash #a #b s x = let x : (_:unit{forall x. b x}) = s in ()
+private
+val revert_squash: #a: Type -> #b: (a -> Type) -> (squash (forall (x: a). b x)) -> x: a ->
+  squash (b x)
+let revert_squash #a #b s x =
+  let x: (_: unit{forall x. b x}) = s in
+  ()
 
-let l_revert () : Tac unit =
-    revert ();
-    apply (`revert_squash)
+let l_revert () : Tac unit = revert (); apply (`revert_squash)
 
-let rec l_revert_all (bs:binders) : Tac unit =
-    match bs with
-    | []    -> ()
-    | _::tl -> begin l_revert (); l_revert_all tl end
+let rec l_revert_all (bs: binders) : Tac unit =
+  match bs with
+  | [] -> ()
+  | _ :: tl -> l_revert (); l_revert_all tl
 
-private val fa_intro_lem : (#a:Type) -> (#p : (a -> Type)) ->
-                           (x:a -> squash (p x)) ->
-                           Lemma (forall (x:a). p x)
+private
+val fa_intro_lem: #a: Type -> #p: (a -> Type) -> (x: a -> squash (p x)) ->
+  Lemma (forall (x: a). p x)
 let fa_intro_lem #a #p f = FStar.Classical.forall_intro #a #p (fun x -> f x <: Lemma (p x))
 
 let forall_intro () : Tac binder =
-    let g = cur_goal () in
-    match term_as_formula g with
-    | Forall _ _ -> begin apply_lemma (`fa_intro_lem); intro () end
-    | _          -> fail "not a forall"
+  let g = cur_goal () in
+  match term_as_formula g with
+  | Forall _ _ -> apply_lemma (`fa_intro_lem); intro ()
+  | _ -> fail "not a forall"
 
-let forall_intro_as (s:string) : Tac binder =
-    let g = cur_goal () in
-    match term_as_formula g with
-    | Forall _ _ -> begin apply_lemma (`fa_intro_lem); intro_as s end
-    | _          -> fail "not a forall"
+let forall_intro_as (s: string) : Tac binder =
+  let g = cur_goal () in
+  match term_as_formula g with
+  | Forall _ _ -> apply_lemma (`fa_intro_lem); intro_as s
+  | _ -> fail "not a forall"
 
 let forall_intros () : Tac binders = repeat1 forall_intro
 
-private val split_lem : (#a:Type) -> (#b:Type) ->
-                        squash a -> squash b -> Lemma (a /\ b)
+private
+val split_lem: #a: Type -> #b: Type -> squash a -> squash b -> Lemma (a /\ b)
 let split_lem #a #b sa sb = ()
 
 let split () : Tac unit =
-    let g = cur_goal () in
-    match term_as_formula g with
-    | And _ _ -> apply_lemma (`split_lem)
-    | _       -> fail "not a conjunction"
+  let g = cur_goal () in
+  match term_as_formula g with
+  | And _ _ -> apply_lemma (`split_lem)
+  | _ -> fail "not a conjunction"
 
-private val imp_intro_lem : (#a:Type) -> (#b : Type) ->
-                            (a -> squash b) ->
-                            Lemma (a ==> b)
+private
+val imp_intro_lem: #a: Type -> #b: Type -> (a -> squash b) -> Lemma (a ==> b)
 let imp_intro_lem #a #b f = FStar.Classical.impl_intro #a #b (fun x -> f x <: Lemma b)
 
 let implies_intro () : Tac binder =
-    let g = cur_goal () in
-    match term_as_formula g with
-    | Implies _ _ -> begin apply_lemma (`imp_intro_lem); intro () end
-    | _           -> fail "not an implication"
+  let g = cur_goal () in
+  match term_as_formula g with
+  | Implies _ _ -> apply_lemma (`imp_intro_lem); intro ()
+  | _ -> fail "not an implication"
 
 let implies_intros () : Tac binders = repeat1 implies_intro
 
-let rec visit (callback:unit -> Tac unit) : Tac unit =
-    focus (fun () ->
-            or_else callback
-                   (fun () ->
-                    let g = cur_goal () in
-                    match term_as_formula g with
-                    | Forall b phi ->
-                        let binders = forall_intros () in
-                        seq (fun () -> visit callback) (fun () -> l_revert_all binders)
-                    | And p q ->
-                        seq split (fun () -> visit callback)
-                    | Implies p q ->
-                        let _ = implies_intro () in
-                        seq (fun () -> visit callback) l_revert
-                    | _ ->
-                        or_else trivial smt
-                   )
-          )
+let rec visit (callback: (unit -> Tac unit)) : Tac unit =
+  focus (fun () ->
+        or_else callback
+          (fun () ->
+              let g = cur_goal () in
+              match term_as_formula g with
+              | Forall b phi ->
+                let binders = forall_intros () in
+                seq (fun () -> visit callback) (fun () -> l_revert_all binders)
+              | And p q -> seq split (fun () -> visit callback)
+              | Implies p q ->
+                let _ = implies_intro () in
+                seq (fun () -> visit callback) l_revert
+              | _ -> or_else trivial smt))
 
 let rec simplify_eq_implication () : Tac unit =
-    let e = cur_env () in
-    let g = cur_goal () in
-    let r = destruct_equality_implication g in
-    match r with
-    | None ->
-        fail "Not an equality implication"
-    | Some (_, rhs) ->
-        let eq_h = implies_intro () in // G, eq_h:x=e |- P
-        rewrite eq_h; // G, eq_h:x=e |- P[e/x]
-        clear_top (); // G |- P[e/x]
-        visit simplify_eq_implication
-
-let rewrite_all_equalities () : Tac unit =
+  let e = cur_env () in
+  let g = cur_goal () in
+  let r = destruct_equality_implication g in
+  match r with
+  | None -> fail "Not an equality implication"
+  | Some (_, rhs) ->
+    // G, eq_h:x=e |- P
+    let eq_h = implies_intro () in
+    // G, eq_h:x=e |- P[e/x]
+    rewrite eq_h;
+    // G |- P[e/x]
+    clear_top ();
     visit simplify_eq_implication
 
-let rec unfold_definition_and_simplify_eq (tm:term) : Tac unit =
-    let g = cur_goal () in
-    match term_as_formula g with
-    | App hd arg ->
-        if term_eq hd tm
-        then trivial ()
-        else ()
-    | _ -> begin
-        let r = destruct_equality_implication g in
-        match r with
-        | None -> fail "Not an equality implication"
-        | Some (_, rhs) ->
-            let eq_h = implies_intro () in
-            rewrite eq_h;
-            clear_top ();
-            visit (fun () -> unfold_definition_and_simplify_eq tm)
-        end
+let rewrite_all_equalities () : Tac unit = visit simplify_eq_implication
 
-private val vbind : (#p:Type) -> (#q:Type) -> squash p -> (p -> squash q) -> Lemma q
+let rec unfold_definition_and_simplify_eq (tm: term) : Tac unit =
+  let g = cur_goal () in
+  match term_as_formula g with
+  | App hd arg -> if term_eq hd tm then trivial ()
+  | _ ->
+    let r = destruct_equality_implication g in
+    match r with
+    | None -> fail "Not an equality implication"
+    | Some (_, rhs) ->
+      let eq_h = implies_intro () in
+      rewrite eq_h;
+      clear_top ();
+      visit (fun () -> unfold_definition_and_simplify_eq tm)
+
+private
+val vbind: #p: Type -> #q: Type -> squash p -> (p -> squash q) -> Lemma q
 let vbind #p #q sq f = FStar.Squash.bind_squash sq f
 
-let unsquash (t:term) : Tac term =
-    let v = `vbind in
-    apply_lemma (mk_e_app v [t]);
-    let b = intro () in
-    pack_ln (Tv_Var (bv_of_binder b))
+let unsquash (t: term) : Tac term =
+  let v = `vbind in
+  apply_lemma (mk_e_app v [t]);
+  let b = intro () in
+  pack_ln (Tv_Var (bv_of_binder b))
 
-let squash_intro () : Tac unit =
-    apply (`FStar.Squash.return_squash)
+let squash_intro () : Tac unit = apply (`FStar.Squash.return_squash)
 
-private val or_ind : (#p:Type) -> (#q:Type) -> (#phi:Type) ->
-                     (p \/ q) ->
-                     (squash (p ==> phi)) ->
-                     (squash (q ==> phi)) ->
-                     Lemma phi
+private
+val or_ind: 
+  #p: Type ->
+  #q: Type ->
+  #phi: Type ->
+  (p \/ q) ->
+  (squash (p ==> phi)) ->
+  (squash (q ==> phi)) ->
+  Lemma phi
 let or_ind #p #q #phi o l r = ()
 
-let cases_or (o:term) : Tac unit =
-    apply_lemma (mk_e_app (`or_ind) [o])
+let cases_or (o: term) : Tac unit = apply_lemma (mk_e_app (`or_ind) [o])
 
-private val bool_ind : (b:bool) -> (phi:Type) -> (squash (b == true  ==> phi)) ->
-                                                 (squash (b == false ==> phi)) ->
-                                                 Lemma phi
+private
+val bool_ind: 
+  b: bool ->
+  phi: Type ->
+  (squash (b == true ==> phi)) ->
+  (squash (b == false ==> phi)) ->
+  Lemma phi
 let bool_ind b phi l r = ()
 
-let cases_bool (b:term) : Tac unit =
-    let bi = `bool_ind in
-    seq (fun () -> apply_lemma (mk_e_app bi [b]))
-        (fun () -> let _ = trytac (fun () -> let b = implies_intro () in rewrite b; clear_top ()) in ())
+let cases_bool (b: term) : Tac unit =
+  let bi = `bool_ind in
+  seq (fun () -> apply_lemma (mk_e_app bi [b]))
+    (fun () ->
+        let _ =
+          trytac (fun () ->
+                let b = implies_intro () in
+                rewrite b;
+                clear_top ())
+        in
+        ())
 
-private val or_intro_1 : (#p:Type) -> (#q:Type) -> squash p -> Lemma (p \/ q)
+private
+val or_intro_1: #p: Type -> #q: Type -> squash p -> Lemma (p \/ q)
 let or_intro_1 #p #q _ = ()
 
-private val or_intro_2 : (#p:Type) -> (#q:Type) -> squash q -> Lemma (p \/ q)
+private
+val or_intro_2: #p: Type -> #q: Type -> squash q -> Lemma (p \/ q)
 let or_intro_2 #p #q _ = ()
 
-let left () : Tac unit =
-    apply_lemma (`or_intro_1)
+let left () : Tac unit = apply_lemma (`or_intro_1)
 
-let right () : Tac unit =
-    apply_lemma (`or_intro_2)
+let right () : Tac unit = apply_lemma (`or_intro_2)
 
-private val __and_elim : (#p:Type) -> (#q:Type) -> (#phi:Type) ->
-                              (p /\ q) ->
-                              squash (p ==> q ==> phi) ->
-                              Lemma phi
+private
+val __and_elim: #p: Type -> #q: Type -> #phi: Type -> (p /\ q) -> squash (p ==> q ==> phi) ->
+  Lemma phi
 let __and_elim #p #q #phi p_and_q f = ()
 
-let and_elim (t : term) : Tac unit =
-    let ae = `__and_elim in
-    apply_lemma (mk_e_app ae [t])
+let and_elim (t: term) : Tac unit =
+  let ae = `__and_elim in
+  apply_lemma (mk_e_app ae [t])
+
