ulib/FStar.UInt32.fst
@@ -1,7 +1,8 @@
 module FStar.UInt32
 (* This module generated automatically using [mk_int.sh] *)
 
-unfold let n = 32
+unfold
+let n = 32
 
 open FStar.UInt
 open FStar.Mul
@@ -15,198 +16,187 @@ open FStar.Mul
  * - some functions (e.g., add_underspec, etc.) are only defined here, not on signed integers
  *)
 
-abstract type t =
-  | Mk: v:uint_t n -> t
+abstract
+type t = | Mk : v: uint_t n -> t
 
 abstract
-let v (x:t) : Tot (uint_t n) = x.v
+let v (x: t) : Tot (uint_t n) = x.v
 
 abstract
-let uint_to_t (x:uint_t n) : Pure t
-  (requires True)
-  (ensures (fun y -> v y = x)) = Mk x
+let uint_to_t (x: uint_t n) : Pure t (requires True) (ensures (fun y -> v y = x)) = Mk x
 
-let uv_inv (x : t) : Lemma
-  (ensures (uint_to_t (v x) == x))
-  [SMTPat (v x)] = ()
+let uv_inv (x: t) : Lemma (ensures (uint_to_t (v x) == x)) [SMTPat (v x)] = ()
 
-let vu_inv (x : uint_t n) : Lemma
-  (ensures (v (uint_to_t x) == x))
-  [SMTPat (uint_to_t x)] = ()
+let vu_inv (x: uint_t n) : Lemma (ensures (v (uint_to_t x) == x)) [SMTPat (uint_to_t x)] = ()
 
-let v_inj (x1 x2: t): Lemma
-  (requires (v x1 == v x2))
-  (ensures (x1 == x2))
-  = ()
+let v_inj (x1: t) (x2: t) : Lemma (requires (v x1 == v x2)) (ensures (x1 == x2)) = ()
 
 abstract
-let add (a:t) (b:t) : Pure t
-  (requires (size (v a + v b) n))
-  (ensures (fun c -> v a + v b = v c))
-  = Mk (add (v a) (v b))
+let add (a: t) (b: t) : Pure t (requires (size (v a + v b) n)) (ensures (fun c -> v a + v b = v c)) =
+  Mk (add (v a) (v b))
 
 abstract
-let add_underspec (a:t) (b:t) : Pure t
-  (requires True)
-  (ensures (fun c ->
-    size (v a + v b) n ==> v a + v b = v c))
- = Mk (add_underspec (v a) (v b))
+let add_underspec (a: t) (b: t)
+  : Pure t (requires True) (ensures (fun c -> size (v a + v b) n ==> v a + v b = v c)) =
+  Mk (add_underspec (v a) (v b))
 
 abstract
-let add_mod (a:t) (b:t) : Pure t
-  (requires True)
-  (ensures (fun c -> FStar.UInt.add_mod (v a) (v b) = v c))
-  = Mk (add_mod (v a) (v b))
+let add_mod (a: t) (b: t)
+  : Pure t (requires True) (ensures (fun c -> FStar.UInt.add_mod (v a) (v b) = v c)) =
+  Mk (add_mod (v a) (v b))
 
 (* Subtraction primitives *)
-abstract
-let sub (a:t) (b:t) : Pure t
-  (requires (size (v a - v b) n))
-  (ensures (fun c -> v a - v b = v c))
-  = Mk (sub (v a) (v b))
 
 abstract
-let sub_underspec (a:t) (b:t) : Pure t
-  (requires True)
-  (ensures (fun c ->
-    size (v a - v b) n ==> v a - v b = v c))
-  = Mk (sub_underspec (v a) (v b))
+let sub (a: t) (b: t) : Pure t (requires (size (v a - v b) n)) (ensures (fun c -> v a - v b = v c)) =
+  Mk (sub (v a) (v b))
 
 abstract
-let sub_mod (a:t) (b:t) : Pure t
-  (requires True)
-  (ensures (fun c -> FStar.UInt.sub_mod (v a) (v b) = v c))
-  = Mk (sub_mod (v a) (v b))
+let sub_underspec (a: t) (b: t)
+  : Pure t (requires True) (ensures (fun c -> size (v a - v b) n ==> v a - v b = v c)) =
+  Mk (sub_underspec (v a) (v b))
+
+abstract
+let sub_mod (a: t) (b: t)
+  : Pure t (requires True) (ensures (fun c -> FStar.UInt.sub_mod (v a) (v b) = v c)) =
+  Mk (sub_mod (v a) (v b))
 
 (* Multiplication primitives *)
-abstract
-let mul (a:t) (b:t) : Pure t
-  (requires (size (v a * v b) n))
-  (ensures (fun c -> v a * v b = v c))
-  = Mk (mul (v a) (v b))
 
 abstract
-let mul_underspec (a:t) (b:t) : Pure t
-  (requires True)
-  (ensures (fun c ->
-    size (v a * v b) n ==> v a * v b = v c))
-   = Mk (mul_underspec (v a) (v b))
+let mul (a: t) (b: t) : Pure t (requires (size (v a * v b) n)) (ensures (fun c -> v a * v b = v c)) =
+  Mk (mul (v a) (v b))
 
 abstract
-let mul_mod (a:t) (b:t) : Pure t
-  (requires True)
-  (ensures (fun c -> FStar.UInt.mul_mod (v a) (v b) = v c))
-  = Mk (mul_mod (v a) (v b))
+let mul_underspec (a: t) (b: t)
+  : Pure t (requires True) (ensures (fun c -> size (v a * v b) n ==> v a * v b = v c)) =
+  Mk (mul_underspec (v a) (v b))
 
 abstract
-let mul_div (a:t) (b:t) : Pure t
-  (requires True)
-  (ensures (fun c -> FStar.UInt.mul_div (v a) (v b) = v c))
-  = Mk (mul_div (v a) (v b))
+let mul_mod (a: t) (b: t)
+  : Pure t (requires True) (ensures (fun c -> FStar.UInt.mul_mod (v a) (v b) = v c)) =
+  Mk (mul_mod (v a) (v b))
+
+abstract
+let mul_div (a: t) (b: t)
+  : Pure t (requires True) (ensures (fun c -> FStar.UInt.mul_div (v a) (v b) = v c)) =
+  Mk (mul_div (v a) (v b))
 
 (* Division primitives *)
+
 abstract
-let div (a:t) (b:t{v b <> 0}) : Pure t
-  (requires (True))
-  (ensures (fun c -> v a / v b = v c))
-  = Mk (div (v a) (v b))
+let div (a: t) (b: t{v b <> 0}) : Pure t (requires (True)) (ensures (fun c -> v a / v b = v c)) =
+  Mk (div (v a) (v b))
 
 (* Modulo primitives *)
+
 abstract
-let rem (a:t) (b:t{v b <> 0}) : Pure t
-  (requires True)
-  (ensures (fun c -> FStar.UInt.mod (v a) (v b) = v c))
-  = Mk (mod (v a) (v b))
+let rem (a: t) (b: t{v b <> 0})
+  : Pure t (requires True) (ensures (fun c -> FStar.UInt.mod (v a) (v b) = v c)) =
+  Mk (mod (v a) (v b))
 
 (* Bitwise operators *)
 
 abstract
-let logand (x:t) (y:t) : Pure t
-  (requires True)
-  (ensures (fun z -> v x `logand` v y = v z))
-  = Mk (logand (v x) (v y))
+let logand (x: t) (y: t) : Pure t (requires True) (ensures (fun z -> logand (v x) (v y) = v z)) =
+  Mk (logand (v x) (v y))
 
 abstract
-let logxor (x:t) (y:t) : Pure t
-  (requires True)
-  (ensures (fun z -> v x `logxor` v y == v z))
-  = Mk (logxor (v x) (v y))
+let logxor (x: t) (y: t) : Pure t (requires True) (ensures (fun z -> logxor (v x) (v y) == v z)) =
+  Mk (logxor (v x) (v y))
 
 abstract
-let logor (x:t) (y:t) : Pure t
-  (requires True)
-  (ensures (fun z -> v x `logor` v y == v z))
-  = Mk (logor (v x) (v y))
+let logor (x: t) (y: t) : Pure t (requires True) (ensures (fun z -> logor (v x) (v y) == v z)) =
+  Mk (logor (v x) (v y))
 
 abstract
-let lognot (x:t) : Pure t
-  (requires True)
-  (ensures (fun z -> lognot (v x) == v z))
-  = Mk (lognot (v x))
+let lognot (x: t) : Pure t (requires True) (ensures (fun z -> lognot (v x) == v z)) =
+  Mk (lognot (v x))
 
 (* Shift operators *)
-abstract
-let shift_right (a:t) (s:t) : Pure t
-  (requires (v s < n))
-  (ensures (fun c -> FStar.UInt.shift_right (v a) (v s) = v c))
-  = Mk (shift_right (v a) (v s))
 
 abstract
-let shift_left (a:t) (s:t) : Pure t
-  (requires (v s < n))
-  (ensures (fun c -> FStar.UInt.shift_left (v a) (v s) = v c))
-  = Mk (shift_left (v a) (v s))
+let shift_right (a: t) (s: t)
+  : Pure t (requires (v s < n)) (ensures (fun c -> FStar.UInt.shift_right (v a) (v s) = v c)) =
+  Mk (shift_right (v a) (v s))
+
+abstract
+let shift_left (a: t) (s: t)
+  : Pure t (requires (v s < n)) (ensures (fun c -> FStar.UInt.shift_left (v a) (v s) = v c)) =
+  Mk (shift_left (v a) (v s))
 
 (* Comparison operators *)
-let eq (a:t) (b:t) : Tot bool = eq #n (v a) (v b)
-let gt (a:t) (b:t) : Tot bool = gt #n (v a) (v b)
-let gte (a:t) (b:t) : Tot bool = gte #n (v a) (v b)
-let lt (a:t) (b:t) : Tot bool = lt #n (v a) (v b)
-let lte (a:t) (b:t) : Tot bool = lte #n (v a) (v b)
+let eq (a: t) (b: t) : Tot bool = eq #n (v a) (v b)
+let gt (a: t) (b: t) : Tot bool = gt #n (v a) (v b)
+let gte (a: t) (b: t) : Tot bool = gte #n (v a) (v b)
+let lt (a: t) (b: t) : Tot bool = lt #n (v a) (v b)
+let lte (a: t) (b: t) : Tot bool = lte #n (v a) (v b)
 
 abstract
-let eq_mask (a:t) (b:t) : Pure t
-  (requires True)
-  (ensures (fun c -> (v a = v b ==> v c = pow2 n - 1) /\
-                  (v a <> v b ==> v c = 0)))
-  = if v a = v b then Mk (pow2 n - 1)
-    else Mk 0
+let eq_mask (a: t) (b: t)
+  : Pure t
+    (requires True)
+    (ensures (fun c -> (v a = v b ==> v c = pow2 n - 1) /\ (v a <> v b ==> v c = 0))) =
+  if v a = v b then Mk (pow2 n - 1) else Mk 0
 
 abstract
-let gte_mask (a:t) (b:t) : Pure t
-  (requires True)
-  (ensures (fun c -> (v a >= v b ==> v c = pow2 n - 1) /\
-                  (v a < v b ==> v c = 0)))
-  = if v a >= v b then Mk (pow2 n - 1)
-    else Mk 0
+let gte_mask (a: t) (b: t)
+  : Pure t
+    (requires True)
+    (ensures (fun c -> (v a >= v b ==> v c = pow2 n - 1) /\ (v a < v b ==> v c = 0))) =
+  if v a >= v b then Mk (pow2 n - 1) else Mk 0
 
 (* Infix notations *)
-unfold let op_Plus_Hat = add
-unfold let op_Plus_Question_Hat = add_underspec
-unfold let op_Plus_Percent_Hat = add_mod
-unfold let op_Subtraction_Hat = sub
-unfold let op_Subtraction_Question_Hat = sub_underspec
-unfold let op_Subtraction_Percent_Hat = sub_mod
-unfold let op_Star_Hat = mul
-unfold let op_Star_Question_Hat = mul_underspec
-unfold let op_Star_Percent_Hat = mul_mod
-unfold let op_Star_Slash_Hat = mul_div
-unfold let op_Slash_Hat = div
-unfold let op_Percent_Hat = rem
-unfold let op_Hat_Hat = logxor
-unfold let op_Amp_Hat = logand
-unfold let op_Bar_Hat = logor
-unfold let op_Less_Less_Hat = shift_left
-unfold let op_Greater_Greater_Hat = shift_right
-unfold let op_Equals_Hat = eq
-unfold let op_Greater_Hat = gt
-unfold let op_Greater_Equals_Hat = gte
-unfold let op_Less_Hat = lt
-unfold let op_Less_Equals_Hat = lte
+unfold
+let op_Plus_Hat = add
+unfold
+let op_Plus_Question_Hat = add_underspec
+unfold
+let op_Plus_Percent_Hat = add_mod
+unfold
+let op_Subtraction_Hat = sub
+unfold
+let op_Subtraction_Question_Hat = sub_underspec
+unfold
+let op_Subtraction_Percent_Hat = sub_mod
+unfold
+let op_Star_Hat = mul
+unfold
+let op_Star_Question_Hat = mul_underspec
+unfold
+let op_Star_Percent_Hat = mul_mod
+unfold
+let op_Star_Slash_Hat = mul_div
+unfold
+let op_Slash_Hat = div
+unfold
+let op_Percent_Hat = rem
+unfold
+let op_Hat_Hat = logxor
+unfold
+let op_Amp_Hat = logand
+unfold
+let op_Bar_Hat = logor
+unfold
+let op_Less_Less_Hat = shift_left
+unfold
+let op_Greater_Greater_Hat = shift_right
+unfold
+let op_Equals_Hat = eq
+unfold
+let op_Greater_Hat = gt
+unfold
+let op_Greater_Equals_Hat = gte
+unfold
+let op_Less_Hat = lt
+unfold
+let op_Less_Equals_Hat = lte
 
 (* To input / output constants *)
-assume val to_string: t -> Tot string
-assume val of_string: string -> Tot t
+assume
+val to_string: t -> Tot string
+assume
+val of_string: string -> Tot t
 
 #set-options "--lax"
 //This private primitive is used internally by the
@@ -216,8 +206,8 @@ assume val of_string: string -> Tot t
 //Since it is marked private, client programs cannot call it directly
 //Since it is marked unfold, it eagerly reduces,
 //eliminating the verification overhead of the wrapper
-private
-unfold
-let __uint_to_t (x:int) : Tot t
-    = uint_to_t x
+
+private unfold
+let __uint_to_t (x: int) : Tot t = uint_to_t x
 #reset-options
+
