ulib/FStar.Exn.fst
@@ -1,4 +1,6 @@
 module FStar.Exn
 
 (* providing the signature of raise, that is implemented natively in FStar_Exn.ml as primitive raise *)
-assume val raise: e:exn -> Exn 'a (requires True) (ensures (fun r -> r == E e))
+assume
+val raise: e: exn -> Exn 'a (requires True) (ensures (fun r -> r == E e))
+
