ulib/FStar.Float.fsti
@@ -1,4 +1,6 @@
 module FStar.Float
 
-assume new type float: Type0
+assume new
+type float : Type0 
 type double = float
+
