ulib/FStar.Heap.fst
@@ -2,8 +2,9 @@ module FStar.Heap
 
 include FStar.Monotonic.Heap
 
-let trivial_rel (a:Type0) :Preorder.relation a = fun x y -> True
+let trivial_rel (a: Type0) : Preorder.relation a = fun x y -> True
 
-let trivial_preorder (a:Type0) :Preorder.preorder a = trivial_rel a
+let trivial_preorder (a: Type0) : Preorder.preorder a = trivial_rel a
 
-type ref (a:Type0) = mref a (trivial_preorder a)
+type ref (a: Type0) = mref a (trivial_preorder a)
+
