ulib/FStar.Mul.fst
@@ -1,4 +1,6 @@
 module FStar.Mul
 //If we're not doing anything with tuples, 
 //open this module to let '*' be multiplication
-unfold let op_Star = Prims.op_Multiply
+unfold
+let op_Star = Prims.op_Multiply
+
