ulib/FStar.PredicateExtensionality.fst
@@ -1,14 +1,13 @@
 module FStar.PredicateExtensionality
 #set-options "--max_fuel 0 --initial_fuel 0 --initial_ifuel 0 --max_ifuel 0"
 
-let predicate (a:Type) = a -> Tot prop
+let predicate (a: Type) = a -> Tot prop
 
-let peq (#a:Type) (p1:predicate a) (p2:predicate a) = forall x. p1 x <==> p2 x
+let peq (#a: Type) (p1: predicate a) (p2: predicate a) = forall x. p1 x <==> p2 x
 
-val predicateExtensionality : a:Type -> p1:predicate a -> p2:predicate a ->
-  Lemma (requires (peq #a p1 p2))
-	(ensures (p1==p2))
-let predicateExtensionality a p1 p2 =  
-  PropositionalExtensionality.axiom();
+val predicateExtensionality: a: Type -> p1: predicate a -> p2: predicate a ->
+  Lemma (requires (peq #a p1 p2)) (ensures (p1 == p2))
+let predicateExtensionality a p1 p2 =
+  PropositionalExtensionality.axiom ();
   assert (FunctionalExtensionality.feq p1 p2)
 
