ulib/FStar.Preorder.fst
@@ -2,14 +2,15 @@ module FStar.Preorder
 
 (* Preordered relations and stable predicates *)
 
-type relation (a:Type) = a -> a -> Type0
+type relation (a: Type) = a -> a -> Type0
 
-type predicate (a:Type) = a -> Type0
+type predicate (a: Type) = a -> Type0
 
-let preorder_rel (#a:Type) (rel:relation a) =
-  (forall (x:a). rel x x) /\ (forall (x:a) (y:a) (z:a). (rel x y /\ rel y z) ==> rel x z)
+let preorder_rel (#a: Type) (rel: relation a) =
+  (forall (x: a). rel x x) /\ (forall (x: a) (y: a) (z: a). (rel x y /\ rel y z) ==> rel x z)
 
-type preorder (a:Type) = rel:relation a{preorder_rel rel}
+type preorder (a: Type) = rel: relation a {preorder_rel rel}
 
-let stable (#a:Type) (p:predicate a) (rel:relation a{preorder_rel rel}) =
-  forall (x:a) (y:a). (p x /\ rel x y) ==> p y
+let stable (#a: Type) (p: predicate a) (rel: relation a {preorder_rel rel}) =
+  forall (x: a) (y: a). (p x /\ rel x y) ==> p y
+
