ulib/FStar.Reflection.Types.fsti
@@ -1,13 +1,21 @@
 module FStar.Reflection.Types
 
-assume new type binder
-assume new type bv
-assume new type term
-assume new type env
-assume new type fv
-assume new type comp
-assume new type sigelt
+assume new
+type binder 
+assume new
+type bv 
+assume new
+type term 
+assume new
+type env 
+assume new
+type fv 
+assume new
+type comp 
+assume new
+type sigelt 
 
 type name : eqtype = list string
-type typ     = term
+type typ = term
 type binders = list binder
+
