ulib/FStar.StrongExcludedMiddle.fst
@@ -1,4 +1,6 @@
 module FStar.StrongExcludedMiddle
 
 (* WARNING: this breaks parametricity; use with care *)
-assume val strong_excluded_middle : p:Type0 -> GTot (b:bool{b = true <==> p})
+assume
+val strong_excluded_middle: p: Type0 -> GTot (b: bool{b = true <==> p})
+
