ulib/FStar.Tactics.Types.fsti
@@ -1,18 +1,21 @@
 module FStar.Tactics.Types
 
-assume new type proofstate
+assume new
+type proofstate 
 
-val incr_depth : proofstate -> proofstate
-val decr_depth : proofstate -> proofstate
-val tracepoint : proofstate -> unit
-val set_proofstate_range : proofstate -> FStar.Range.range -> proofstate
+val incr_depth: proofstate -> proofstate
+val decr_depth: proofstate -> proofstate
+val tracepoint: proofstate -> unit
+val set_proofstate_range: proofstate -> FStar.Range.range -> proofstate
 
 type direction =
-    | TopDown
-    | BottomUp
+  | TopDown
+  | BottomUp
 
 type guard_policy =
-    | SMT
-    | Goal
-    | Force
-    | Drop // unsound! careful!
+  | SMT
+  | Goal
+  | Force
+  // unsound! careful!
+  | Drop
+
